Many changes including redefinition of program transformation and proofmode for [sim]. Backup before splitting well-formedness in two.

theories/language/well_formed.v
@@ -20,7 +20,7 @@ Fixpoint expr_well_formed prog lvl e :=
   | Val v =>
       val_well_formed prog v
   | Var x =>
-      x ≤ lvl
+      x < lvl
   | Let e1 e2 =>
       expr_well_formed prog lvl e1 ∧
       expr_well_formed prog (S lvl) e2
@@ -54,10 +54,10 @@ Definition expr_well_formed' prog e :=
   ∃ lvl, expr_well_formed prog lvl e.
 
 Definition program_well_formed prog :=
-  map_Forall (λ _, expr_well_formed prog 0) prog.
+  map_Forall (λ _, expr_well_formed prog 1) prog.
 
-Lemma expr_well_formed_subst ς1 ς2 prog lvl e :
-  (∀ x, x ≤ lvl → ς1 x = ς2 x) →
+Lemma subst_expr_well_formed ς1 ς2 prog lvl e :
+  (∀ x, x < lvl → ς1 x = ς2 x) →
   expr_well_formed prog lvl e →
   e.[ς1] = e.[ς2].
 Proof.
@@ -81,23 +81,107 @@ Proof.
   eapply IHe2; last naive_solver.
   intros x Hx. destruct x; first done. asimpl. f_equal. naive_solver lia.
 Qed.
-Lemma expr_well_formed_0_subst ς1 ς2 prog e :
-  ς1 0 = ς2 0 →
+Lemma subst_expr_well_formed_0 ς1 ς2 prog e :
   expr_well_formed prog 0 e →
   e.[ς1] = e.[ς2].
 Proof.
-  intros Hς Hwf.
-  eapply expr_well_formed_subst; last done.
-  setoid_rewrite Nat.le_0_r. naive_solver.
+  intros Hwf.
+  eapply subst_expr_well_formed; last done.
+  lia.
 Qed.
-
-Lemma program_well_formed_subst ς1 ς2 prog func e :
+Lemma subst_expr_well_formed_1 ς1 ς2 prog e :
+  ς1 0 = ς2 0 →
+  expr_well_formed prog 1 e →
+  e.[ς1] = e.[ς2].
+Proof.
+  intros Hς Hwf.
+  eapply subst_expr_well_formed; last done.
+  setoid_rewrite Nat.lt_1_r. naive_solver.
+Qed.
+Lemma subst_expr_well_formed_1' ς1 ς2 v prog e :
+  expr_well_formed prog 1 e →
+  e.[v .: ς1] = e.[v .: ς2].
+Proof.
+  apply subst_expr_well_formed_1. done.
+Qed.
+Lemma subst_program_well_formed ς1 ς2 prog func e :
   ς1 0 = ς2 0 →
   program_well_formed prog →
   prog !! func = Some e →
   e.[ς1] = e.[ς2].
 Proof.
   intros Hσ Hwf Hlookup.
-  eapply expr_well_formed_0_subst; first done.
+  eapply subst_expr_well_formed_1; first done.
   pose proof (map_Forall_lookup_1 _ _ _ _ Hwf Hlookup). eauto.
+Qed.
+Lemma subst_program_well_formed' ς1 ς2 v prog func e :
+  program_well_formed prog →
+  prog !! func = Some e →
+  e.[v .: ς1] = e.[v .: ς2].
+Proof.
+  apply subst_program_well_formed. done.
+Qed.
+
+Lemma expr_well_formed_le prog lvl1 lvl2 e :
+  lvl1 ≤ lvl2 →
+  expr_well_formed prog lvl1 e →
+  expr_well_formed prog lvl2 e.
+Proof.
+  revert lvl1 lvl2. elim e; try naive_solver lia.
+  intros e1 IH1 e2 IH2 lvl1 lvl2 Hlvl (Hwf1 & Hwf2).
+  split; first naive_solver. eapply IH2; last done. lia.
+Qed.
+
+Lemma expr_well_formed_upn_subst_val n v prog lvl e :
+  n < lvl →
+  val_well_formed prog v →
+  expr_well_formed prog lvl e →
+  expr_well_formed prog (lvl - 1) e.[upn n (Val v .: ids)].
+Proof.
+  revert n lvl. induction e; intros n lvl; try naive_solver; simpl.
+  - intros Hn Hv Hx.
+    destruct (Nat.lt_ge_cases x n) as [Hx' | (dx & ->)%Nat.le_sum].
+    + rewrite upn_lt //=. lia.
+    + rewrite upn_ge; first lia.
+      rewrite Nat.sub_add'. destruct dx; first done. simpl. lia.
+  - intros Hn Hv (Hwf1 & Hwf2). split; first naive_solver.
+    rewrite fold_up_upn.
+    destruct lvl; first lia.
+    rewrite /= Nat.sub_0_r -(Nat.pred_succ (S lvl)) -Nat.sub_1_r.
+    auto with lia.
+Qed.
+Lemma expr_well_formed_subst_val prog lvl e v :
+  val_well_formed prog v →
+  expr_well_formed prog lvl e →
+  expr_well_formed prog (lvl - 1) e.[Val v/].
+Proof.
+  destruct lvl.
+  - intros Hv Hwf%(expr_well_formed_le _ _ 1)%(expr_well_formed_upn_subst_val 0 v); naive_solver lia.
+  - apply (expr_well_formed_upn_subst_val 0). lia.
+Qed.
+
+Lemma expr_well_formed_ren ξ n prog lvl e :
+  (∀ x, ξ x ≤ x + n) →
+  expr_well_formed prog lvl e →
+  expr_well_formed prog (lvl + n) e.[ren ξ].
+Proof.
+  revert lvl ξ n. elim e; try naive_solver lia.
+  - intros x lvl ξ n Hξ Hwf.
+    eapply (Nat.le_lt_trans _ (x + n)); naive_solver lia.
+  - intros e1 IH1 e2 IH2 lvl ξ n Hξ (Hwf1 & Hwf2).
+    split; first naive_solver.
+    asimpl. rewrite -Nat.add_succ_l. apply IH2; last done.
+    intros []; simpl; [lia | rewrite -Nat.succ_le_mono //].
+Qed.
+Lemma expr_well_formed_lift n prog lvl e :
+  expr_well_formed prog lvl e →
+  expr_well_formed prog (lvl + n) e.[ren (+n)].
+Proof.
+  apply expr_well_formed_ren. naive_solver lia.
+Qed.
+Lemma expr_well_formed_lift1 prog lvl e :
+  expr_well_formed prog lvl e →
+  expr_well_formed prog (S lvl) e.[ren (+1)].
+Proof.
+  rewrite -Nat.add_1_r. apply expr_well_formed_lift.
 Qed.
