theories/common/autosubst.v
@@ -1,0 +1,29 @@
+From Autosubst Require Export
+  Autosubst.
+
+From simuliris Require Export
+  prelude.
+
+Section subst.
+  Context `{!Ids term, !Rename term, !Subst term, !SubstLemmas term}.
+  Implicit Types x : var.
+  Implicit Types ς : var → term.
+
+  Lemma upn_lt x n ς :
+    x < n →
+    upn n ς x = ids x.
+  Proof.
+    revert x. induction n; intros x Hx; first lia.
+    rewrite upnSE. destruct x; first done.
+    rewrite /= IHn; [lia | autosubst].
+  Qed.
+  Lemma upn_ge x n ς :
+    n ≤ x →
+    upn n ς x = (ς (x - n)).[ren (+n)].
+  Proof.
+    revert x. induction n; intros x Hx.
+    - rewrite upn0 Nat.sub_0_r. autosubst.
+    - rewrite upnSE. destruct x; first lia.
+      asimpl. rewrite IHn; first lia. autosubst.
+  Qed.
+End subst.
