theories/common/fin_maps.v
@@ -1,0 +1,352 @@
+From stdpp Require Export
+  fin_maps.
+
+(* FIXME: This file needs a 'Proof Using' hint, but they need to be set
+locally (or things moved out of sections) as no default works well enough. *)
+Unset Default Proof Using.
+
+(** Given a finite map [m : M] with keys [K] and values [A], the image [map_img m]
+gives a finite set containing with the values [A] of [m]. The type of [map_img]
+is generic to support different map and set implementations. A possible instance
+is [SA:=gset A]. *)
+Definition map_img `{FinMapToList K A M,
+  Singleton A SA, Empty SA, Union SA} : M → SA := map_to_set (λ _ x, x).
+Global Typeclasses Opaque map_img.
+
+(** Given a finite map [m] with keys [K] and values [A], the preimage
+[map_preimg m] gives a finite map with keys [A] and values being sets of [K].
+The type of [map_preimg] is very generic to support different map and set
+implementations. A possible instance is [MKA:=gmap K A], [MASK:=gmap A (gset K)],
+and [SK:=gset K]. *)
+Definition map_preimg `{FinMapToList K A MKA, Empty MASK,
+    PartialAlter A SK MASK, Empty SK, Singleton K SK, Union SK}
+    (m : MKA) : MASK :=
+  map_fold (λ i, partial_alter (λ mX, Some $ {[ i ]} ∪ default ∅ mX)) ∅ m.
+Global Typeclasses Opaque map_preimg.
+
+Section preimg.
+  (** We restrict the theory to finite sets with Leibniz equality, which is
+  sufficient for [gset], but not for [boolset] or [propset]. The result of the
+  pre-image is a map of sets. To support general sets, we would need setoid
+  equality on sets, and thus setoid equality on maps. *)
+  Context `{FinMap K MK, FinMap A MA, FinSet K SK, !LeibnizEquiv SK}.
+  Local Notation map_preimg :=
+    (map_preimg (K:=K) (A:=A) (MKA:=MK A) (MASK:=MA SK) (SK:=SK)).
+  Implicit Types m : MK A.
+
+  Lemma map_preimg_empty : map_preimg ∅ = ∅.
+  Proof. apply map_fold_empty. Qed.
+  Lemma map_preimg_insert m i x :
+    m !! i = None →
+    map_preimg (<[i:=x]> m) =
+      partial_alter (λ mX, Some ({[ i ]} ∪ default ∅ mX)) x (map_preimg m).
+  Proof.
+    intros Hi. refine (map_fold_insert_L _ _ i x m _ Hi).
+    intros j1 j2 x1 x2 m' ? _ _. destruct (decide (x1 = x2)) as [->|?].
+    - rewrite <-!partial_alter_compose.
+      apply partial_alter_ext; intros ? _; f_equal/=. set_solver.
+    - by apply partial_alter_commute.
+  Qed.
+
+  (** The [map_preimg] function never returns an empty set (we represent that
+  case via [None]). *)
+  Lemma lookup_preimg_Some_non_empty m x :
+    map_preimg m !! x ≠ Some ∅.
+  Proof.
+    induction m as [|i x' m ? IH] using map_ind.
+    { by rewrite map_preimg_empty, lookup_empty. }
+    rewrite map_preimg_insert by done. destruct (decide (x = x')) as [->|].
+    - rewrite lookup_partial_alter. intros [=]. set_solver.
+    - rewrite lookup_partial_alter_ne by done. set_solver.
+  Qed.
+
+  Lemma lookup_preimg_None_1 m x i :
+    map_preimg m !! x = None → m !! i ≠ Some x.
+  Proof.
+    induction m as [|i' x' m ? IH] using map_ind; [by rewrite lookup_empty|].
+    rewrite map_preimg_insert by done. destruct (decide (x = x')) as [->|].
+    - by rewrite lookup_partial_alter.
+    - rewrite lookup_partial_alter_ne, lookup_insert_Some by done. naive_solver.
+  Qed.
+
+  Lemma lookup_preimg_Some_1 m X x i :
+    map_preimg m !! x = Some X →
+    i ∈ X ↔ m !! i = Some x.
+  Proof.
+    revert X. induction m as [|i' x' m ? IH] using map_ind; intros X.
+    { by rewrite map_preimg_empty, lookup_empty. }
+    rewrite map_preimg_insert by done. destruct (decide (x = x')) as [->|].
+    - rewrite lookup_partial_alter. intros [= <-].
+      rewrite elem_of_union, elem_of_singleton, lookup_insert_Some.
+      destruct (map_preimg m !! x') as [X'|] eqn:Hx'; simpl.
+      + rewrite IH by done. naive_solver.
+      + apply (lookup_preimg_None_1 _ _ i) in Hx'. set_solver.
+    - rewrite lookup_partial_alter_ne, lookup_insert_Some by done. naive_solver.
+  Qed.
+
+  Lemma lookup_preimg_None m x :
+    map_preimg m !! x = None ↔ ∀ i, m !! i ≠ Some x.
+  Proof.
+    split; [by eauto using lookup_preimg_None_1|].
+    intros Hm. apply eq_None_not_Some; intros [X ?].
+    destruct (set_choose_L X) as [i ?].
+    { intros ->. by eapply lookup_preimg_Some_non_empty. }
+    by eapply (Hm i), lookup_preimg_Some_1.
+  Qed.
+
+  Lemma lookup_preimg_Some m x X :
+    map_preimg m !! x = Some X ↔ X ≠ ∅ ∧ ∀ i, i ∈ X ↔ m !! i = Some x.
+  Proof.
+    split.
+    - intros HxX. split; [intros ->; by eapply lookup_preimg_Some_non_empty|].
+      intros j. by apply lookup_preimg_Some_1.
+    - intros [HXne HX]. destruct (map_preimg m !! x) as [X'|] eqn:HX'.
+      + f_equal; apply set_eq; intros i. rewrite HX.
+        by apply lookup_preimg_Some_1.
+      + apply set_choose_L in HXne as [j ?].
+        apply (lookup_preimg_None_1 _ _ j) in HX'. naive_solver.
+  Qed.
+
+  Lemma lookup_total_preimg m x i :
+    i ∈ map_preimg m !!! x ↔ m !! i = Some x.
+  Proof.
+    rewrite lookup_total_alt. destruct (map_preimg m !! x) as [X|] eqn:HX.
+    - by apply lookup_preimg_Some.
+    - rewrite lookup_preimg_None in HX. set_solver.
+  Qed.
+End preimg.
+
+(** ** The [map_img] (image/codomain) operation *)
+Section img.
+  Context `{FinMap K M, FinSet A SA}.
+  Implicit Types m : M A.
+  Implicit Types x y : A.
+  Implicit Types X : SA.
+
+  (* avoid writing ≡@{D} everywhere... *)
+  Notation map_img := (map_img (M:=M A) (SA:=SA)).
+
+  Lemma elem_of_map_img m x : x ∈ map_img m ↔ ∃ i, m !! i = Some x.
+  Proof. unfold map_img. rewrite @elem_of_map_to_set; try apply _. naive_solver. Qed.
+  Lemma elem_of_map_img_1 m x : x ∈ map_img m → ∃ i, m !! i = Some x.
+  Proof. apply elem_of_map_img. Qed.
+  Lemma elem_of_map_img_2 m i x : m !! i = Some x → x ∈ map_img m.
+  Proof. rewrite elem_of_map_img. eauto. Qed.
+
+  Lemma not_elem_of_map_img m x : x ∉ map_img m ↔ ∀ i, m !! i ≠ Some x.
+  Proof. rewrite elem_of_map_img. naive_solver. Qed.
+  Lemma not_elem_of_map_img_1 m i x : x ∉ map_img m → m !! i ≠ Some x.
+  Proof. rewrite not_elem_of_map_img. eauto. Qed.
+  Lemma not_elem_of_map_img_2 m x : (∀ i, m !! i ≠ Some x) → x ∉ map_img m.
+  Proof. apply not_elem_of_map_img. Qed.
+
+  Lemma map_subseteq_img m1 m2 : m1 ⊆ m2 → map_img m1 ⊆ map_img m2.
+  Proof.
+    rewrite map_subseteq_spec. intros ? x.
+    rewrite !elem_of_map_img. naive_solver.
+  Qed.
+
+  Lemma map_img_filter (P : K * A → Prop) `{!∀ ix, Decision (P ix)} m X :
+    (∀ x, x ∈ X ↔ ∃ i, m !! i = Some x ∧ P (i, x)) →
+    map_img (filter P m) ≡ X.
+  Proof.
+    intros HX x. rewrite elem_of_map_img, HX.
+    unfold is_Some. by setoid_rewrite map_filter_lookup_Some.
+  Qed.
+  Lemma map_img_filter_subseteq (P : K * A → Prop) `{!∀ ix, Decision (P ix)} m :
+    map_img (filter P m) ⊆ map_img m.
+  Proof. apply map_subseteq_img, map_filter_subseteq. Qed.
+
+  Lemma map_img_empty : map_img ∅ ≡ ∅.
+  Proof.
+    rewrite set_equiv. intros x. rewrite elem_of_map_img, elem_of_empty.
+    setoid_rewrite lookup_empty. naive_solver.
+  Qed.
+  Lemma map_img_empty_iff m : map_img m ≡ ∅ ↔ m = ∅.
+  Proof.
+    split; [|intros ->; by rewrite map_img_empty].
+    intros Hm. apply map_empty; intros i.
+    apply eq_None_ne_Some; intros x ?%elem_of_map_img_2. set_solver.
+  Qed.
+  Lemma map_img_empty_inv m : map_img m ≡ ∅ → m = ∅.
+  Proof. apply map_img_empty_iff. Qed.
+
+  Lemma map_img_delete_subseteq i m : map_img (delete i m) ⊆ map_img m.
+  Proof. apply map_subseteq_img, delete_subseteq. Qed.
+
+  Lemma map_img_insert m i x :
+    map_img (<[i:=x]> m) ≡ {[ x ]} ∪ map_img (delete i m).
+  Proof.
+    intros y. rewrite elem_of_union, !elem_of_map_img, elem_of_singleton.
+    setoid_rewrite lookup_delete_Some. setoid_rewrite lookup_insert_Some.
+    naive_solver.
+  Qed.
+  Lemma map_img_insert_notin m i x :
+    m !! i = None → map_img (<[i:=x]> m) ≡ {[ x ]} ∪ map_img m.
+  Proof. intros. by rewrite map_img_insert, delete_notin. Qed.
+
+  Lemma map_img_insert_subseteq m i x :
+    map_img (<[i:=x]> m) ⊆ {[ x ]} ∪ map_img m.
+  Proof.
+    rewrite map_img_insert. apply union_mono_l, map_img_delete_subseteq.
+  Qed.
+  Lemma elem_of_map_img_insert m i x : x ∈ map_img (<[i:=x]> m).
+  Proof. apply elem_of_map_img. exists i. apply lookup_insert. Qed.
+  Lemma elem_of_map_img_insert_ne m i x y :
+    x ≠ y → x ∈ map_img (<[i:=y]> m) → x ∈ map_img m.
+  Proof. intros ? ?%map_img_insert_subseteq. set_solver. Qed.
+
+  Lemma map_img_singleton i x : map_img {[ i := x ]} ≡ {[ x ]}.
+  Proof.
+    apply set_equiv. intros y.
+    rewrite elem_of_map_img. setoid_rewrite lookup_singleton_Some. set_solver.
+  Qed.
+
+  Lemma elem_of_map_img_union m1 m2 x :
+    x ∈ map_img (m1 ∪ m2) →
+    x ∈ map_img m1 ∨ x ∈ map_img m2.
+  Proof.
+    rewrite !elem_of_map_img. setoid_rewrite lookup_union_Some_raw. naive_solver.
+  Qed.
+  Lemma elem_of_map_img_union_l m1 m2 x :
+    x ∈ map_img m1 → x ∈ map_img (m1 ∪ m2).
+  Proof.
+    rewrite !elem_of_map_img. setoid_rewrite lookup_union_Some_raw. naive_solver.
+  Qed.
+  Lemma elem_of_map_img_union_r m1 m2 x :
+    m1 ##ₘ m2 → x ∈ map_img m2 → x ∈ map_img (m1 ∪ m2).
+  Proof.
+    intros. rewrite map_union_comm by done. by apply elem_of_map_img_union_l.
+  Qed.
+  Lemma elem_of_map_img_union_disjoint m1 m2 x :
+    m1 ##ₘ m2 → x ∈ map_img (m1 ∪ m2) ↔ x ∈ map_img m1 ∨ x ∈ map_img m2.
+  Proof.
+    naive_solver eauto using elem_of_map_img_union,
+      elem_of_map_img_union_l, elem_of_map_img_union_r.
+  Qed.
+
+  Lemma map_img_union_subseteq m1 m2 :
+    map_img (m1 ∪ m2) ⊆ map_img m1 ∪ map_img m2.
+  Proof. intros v Hv. apply elem_of_union, elem_of_map_img_union. exact Hv. Qed.
+  Lemma map_img_union_subseteq_l m1 m2 : map_img m1 ⊆ map_img (m1 ∪ m2).
+  Proof. intros v Hv. by apply elem_of_map_img_union_l. Qed.
+  Lemma map_img_union_subseteq_r m1 m2 :
+    m1 ##ₘ m2 → map_img m2 ⊆ map_img (m1 ∪ m2).
+  Proof. intros Hdisj v Hv. by apply elem_of_map_img_union_r. Qed.
+  Lemma map_img_union_disjoint m1 m2 :
+    m1 ##ₘ m2 → map_img (m1 ∪ m2) ≡ map_img m1 ∪ map_img m2.
+  Proof.
+    intros Hdisj. apply set_equiv. intros x.
+    rewrite elem_of_union. by apply elem_of_map_img_union_disjoint.
+  Qed.
+
+  Lemma map_img_finite m : set_finite (map_img m).
+  Proof.
+    induction m as [|i x m ? IH] using map_ind.
+    - rewrite map_img_empty. apply empty_finite.
+    - eapply set_finite_subseteq; [by apply map_img_insert_subseteq|].
+      apply union_finite; [apply singleton_finite | apply IH].
+  Qed.
+
+  (** Alternative definition of [img] in terms of [map_to_list]. *)
+  Lemma map_img_alt m : map_img m ≡ list_to_set (map_to_list m).*2.
+  Proof.
+    induction m as [|i x m ? IH] using map_ind.
+    { by rewrite map_img_empty, map_to_list_empty. }
+    by rewrite map_img_insert_notin, map_to_list_insert by done.
+  Qed.
+
+  Lemma map_img_singleton_inv m i x :
+    map_img m ≡ {[ x ]} → m !! i = None ∨ m !! i = Some x.
+  Proof.
+    intros Hm. destruct (m !! i) eqn:Hmk; [|by auto].
+    apply elem_of_map_img_2 in Hmk. set_solver.
+  Qed.
+
+  Lemma map_img_union_inv `{!RelDecision (∈@{SA})} X Y m :
+    X ## Y →
+    map_img m ≡ X ∪ Y →
+    ∃ m1 m2, m = m1 ∪ m2 ∧ m1 ##ₘ m2 ∧ map_img m1 ≡ X ∧ map_img m2 ≡ Y.
+  Proof.
+    intros Hsep Himg.
+    exists (filter (λ '(_,x), x ∈ X) m), (filter (λ '(_,x), x ∉ X) m).
+    assert (filter (λ '(_,x), x ∈ X) m ##ₘ filter (λ '(_,x), x ∉ X) m).
+    { apply map_disjoint_filter_complement. }
+    split_and!.
+    - symmetry. apply map_filter_union_complement.
+    - done.
+    - apply map_img_filter; intros x. split; [|naive_solver].
+      intros. destruct (elem_of_map_img_1 m x); set_solver.
+    - apply map_img_filter; intros x; split.
+      + intros. destruct (elem_of_map_img_1 m x); set_solver.
+      + intros (i & ?%elem_of_map_img_2 & ?). set_solver.
+  Qed.
+
+  Section leibniz.
+    Context `{!LeibnizEquiv SA}.
+
+    Lemma map_img_empty_L : map_img ∅ = ∅.
+    Proof. unfold_leibniz. exact map_img_empty. Qed.
+
+    Lemma map_img_empty_iff_L m : map_img m = ∅ ↔ m = ∅.
+    Proof. unfold_leibniz. apply map_img_empty_iff. Qed.
+    Lemma map_img_empty_inv_L m : map_img m = ∅ → m = ∅.
+    Proof. apply map_img_empty_iff_L. Qed.
+
+    Lemma map_img_singleton_L i x : map_img {[ i := x ]} = {[ x ]}.
+    Proof. unfold_leibniz. apply map_img_singleton. Qed.
+
+    Lemma map_img_insert_notin_L m i x :
+      m !! i = None → map_img (<[i:=x]> m) = {[ x ]} ∪ map_img m.
+    Proof. unfold_leibniz. apply map_img_insert_notin. Qed.
+
+    Lemma map_img_union_disjoint_L m1 m2 :
+      m1 ##ₘ m2 → map_img (m1 ∪ m2) = map_img m1 ∪ map_img m2.
+    Proof. unfold_leibniz. apply map_img_union_disjoint. Qed.
+
+    Lemma map_img_alt_L m : map_img m = list_to_set (map_to_list m).*2.
+    Proof. unfold_leibniz. apply map_img_alt. Qed.
+
+    Lemma map_img_singleton_inv_L m i x :
+      map_img m = {[ x ]} → m !! i = None ∨ m !! i = Some x.
+    Proof. unfold_leibniz. apply map_img_singleton_inv. Qed.
+
+    Lemma map_img_union_inv_L `{!RelDecision (∈@{SA})} X Y m :
+      X ## Y →
+      map_img m = X ∪ Y →
+      ∃ m1 m2, m = m1 ∪ m2 ∧ m1 ##ₘ m2 ∧ map_img m1 = X ∧ map_img m2 = Y.
+    Proof. unfold_leibniz. apply map_img_union_inv. Qed.
+  End leibniz.
+
+  (** * Set solver instances *)
+  Global Instance set_unfold_map_img_empty x :
+    SetUnfoldElemOf x (map_img (∅:M A)) False.
+  Proof. constructor. by rewrite map_img_empty, elem_of_empty. Qed.
+  Global Instance set_unfold_map_img_singleton x i y :
+    SetUnfoldElemOf x (map_img ({[i:=y]}:M A)) (x = y).
+  Proof. constructor. by rewrite map_img_singleton, elem_of_singleton. Qed.
+End img.
+
+Lemma map_img_fmap `{FinMap K M, FinSet A SA, FinSet B SB} (f : A → B) (m : M A) :
+  map_img (f <$> m) ≡@{SB} set_map (C:=SA) f (map_img m).
+Proof.
+  apply set_equiv. intros y. rewrite elem_of_map_img, elem_of_map.
+  setoid_rewrite lookup_fmap. setoid_rewrite fmap_Some.
+  setoid_rewrite elem_of_map_img. naive_solver.
+Qed.
+Lemma map_img_fmap_L `{FinMap K M, FinSet A SA, FinSet B SB, !LeibnizEquiv SB}
+    (f : A → B) (m : M A) :
+  map_img (f <$> m) =@{SB} set_map (C:=SA) f (map_img m).
+Proof. unfold_leibniz. apply map_img_fmap. Qed.
+
+Lemma map_img_kmap `{FinMap K M, FinMap K2 M2, FinSet A SA}
+    (f : K → K2) `{!Inj (=) (=) f} m :
+  map_img (kmap (M2:=M2) f m) ≡@{SA} map_img m.
+Proof.
+  apply set_equiv. intros x. rewrite !elem_of_map_img.
+  setoid_rewrite (lookup_kmap_Some f). naive_solver.
+Qed.
+Lemma map_img_kmap_L `{FinMap K M, FinMap K2 M2, FinSet A SA, !LeibnizEquiv SA}
+    (f : K → K2) `{!Inj (=) (=) f} m :
+  map_img (kmap (M2:=M2) f m) =@{SA} map_img m.
+Proof. unfold_leibniz. by apply map_img_kmap. Qed.
