theories/program_logic/sim/definition.v
@@ -8,73 +8,76 @@ From simuliris.base_logic Require Export
 From simuliris.program_logic Require Export
   sim.protocol.
 
-Class SimState PROP Λₛ Λₜ := {
-  sim_state_interp : state Λₛ → state Λₜ → PROP ;
-}.
-#[global] Arguments Build_SimState {_ _ _} _ : assert.
-
 Class SimPrograms Λₛ Λₜ := {
   sim_progₛ : program Λₛ ;
   sim_progₜ : program Λₜ ;
 }.
 #[global] Arguments Build_SimPrograms {_ _} _ _ : assert.
 
-Section sim.
+Class SimState PROP Λₛ Λₜ := {
+  sim_state_interp : state Λₛ → state Λₜ → PROP ;
+}.
+#[global] Arguments Build_SimState {_ _ _} _ : assert.
+
+Section sim_cupd.
   Context `{!BiBUpd PROP, !BiAffine PROP}.
   Context `{sim_state : !SimState PROP Λₛ Λₜ}.
+
+  #[local] Definition sim_cupd : CUpd PROP := (
+    λ P,
+      ∀ σₛ σₜ,
+      sim_state_interp σₛ σₜ ==∗
+      sim_state_interp σₛ σₜ ∗ P
+  )%I.
+  #[global] Program Instance sim_bi_cupd : BiCUpd PROP :=
+    Build_BiCUpd sim_cupd _.
+  Next Obligation.
+    split; rewrite /cupd /sim_cupd.
+    - solve_proper.
+    - auto with iFrame.
+    - iIntros "%P %Q %HPQ HP * Hsi".
+      iMod ("HP" with "Hsi") as "(Hsi & HP)".
+      iFrame. iApply (HPQ with "HP").
+    - iIntros "%P HP * Hsi".
+      do 2 iMod ("HP" with "Hsi") as "(Hsi & HP)".
+      iFrame. done.
+    - iIntros "%P %R (HP & HR) * Hsi".
+      iMod ("HP" with "Hsi") as "(Hsi & HP)".
+      iFrame. done.
+    - iIntros "%P HP * Hsi". iFrame.
+  Qed.
+
+  Lemma sim_cupd_eq P :
+    (|++> P) ⊣⊢
+    ∀ σₛ σₜ,
+    sim_state_interp σₛ σₜ ==∗
+    sim_state_interp σₛ σₜ ∗
+    P.
+  Proof.
+    done.
+  Qed.
+
+  (* FIXME: we should not need this *)
+  #[global] Instance sim_cupd_ne :
+    NonExpansive (sim_cupd).
+  Proof.
+    apply (@cupd_ne _ _ sim_bi_cupd).
+  Qed.
+End sim_cupd.
+
+#[global] Opaque sim_cupd.
+
+Section sim.
+  Context `{sim_programs : !SimPrograms Λₛ Λₜ}.
+  Context `{!BiBUpd PROP, !BiAffine PROP}.
+  Context `{sim_state : !SimState PROP Λₛ Λₜ}.
+  Context (X : sim_protocol PROP Λₛ Λₜ).
 
   Notation expr_relation :=
     (expr Λₛ → expr Λₜ → PROP).
   Notation expr_relation_O :=
     (expr_O Λₛ -d> expr_O Λₜ -d> PROP).
 
-  Section sim_cupd.
-    #[local] Definition sim_cupd : CUpd PROP := (
-      λ P,
-        ∀ σₛ σₜ,
-        sim_state_interp σₛ σₜ ==∗
-        sim_state_interp σₛ σₜ ∗ P
-    )%I.
-    #[global] Program Instance sim_bi_cupd : BiCUpd PROP :=
-      Build_BiCUpd sim_cupd _.
-    Next Obligation.
-      split; rewrite /cupd /sim_cupd.
-      - solve_proper.
-      - auto with iFrame.
-      - iIntros "%P %Q %HPQ HP * Hsi".
-        iMod ("HP" with "Hsi") as "(Hsi & HP)".
-        iFrame. iApply (HPQ with "HP").
-      - iIntros "%P HP * Hsi".
-        do 2 iMod ("HP" with "Hsi") as "(Hsi & HP)".
-        iFrame. done.
-      - iIntros "%P %R (HP & HR) * Hsi".
-        iMod ("HP" with "Hsi") as "(Hsi & HP)".
-        iFrame. done.
-      - iIntros "%P HP * Hsi". iFrame.
-    Qed.
-
-    Lemma sim_cupd_eq P :
-      (|++> P) ⊣⊢
-      ∀ σₛ σₜ,
-      sim_state_interp σₛ σₜ ==∗
-      sim_state_interp σₛ σₜ ∗
-      P.
-    Proof.
-      done.
-    Qed.
-
-    (* FIXME: we should not need this *)
-    #[global] Instance sim_cupd_ne :
-      NonExpansive (sim_cupd).
-    Proof.
-      apply (@cupd_ne _ _ sim_bi_cupd).
-    Qed.
-  End sim_cupd.
-
-  #[global] Opaque sim_cupd.
-
-  Context `{sim_programs : !SimPrograms Λₛ Λₜ}.
-  Context (X : sim_protocol PROP Λₛ Λₜ).
   Implicit Types N M I : sim_protocol_O PROP Λₛ Λₜ.
   Implicit Types R : expr_relation_O → expr_relation_O → PROP.
 
