theories/program_logic/sim/proofmode.v
@@ -11,331 +11,563 @@ From simuliris.program_logic Require Export
 From simuliris.program_logic Require Import
   sim.notations.
 
-Section sim.
+Section sim_state.
+  Context `{sim_programs : !SimPrograms Λₛ Λₜ}.
   Context `{!BiBUpd PROP, !BiAffine PROP}.
   Context `{sim_state : !SimState PROP Λₛ Λₜ}.
-  Context `{sim_programs : !SimPrograms Λₛ Λₜ}.
   Context (X : sim_protocol PROP Λₛ Λₜ).
 
-  #[global] Instance frame_simv p R eₛ eₜ Φ1 Φ2 :
-    (∀ eₛ eₜ, Frame p R (Φ1 eₛ eₜ) (Φ2 eₛ eₜ)) →
-    Frame p R
-      (SIM eₛ ≳ eₜ [[ X ]] [[ Φ1 ]])
-      (SIM eₛ ≳ eₜ [[ X ]] [[ Φ2 ]]).
-  Proof.
-    rewrite /Frame simv_frame_l.
-    iIntros "%HR Hsim".
-    iApply (simv_mono with "[] Hsim"). iIntros "%eₛ' %eₜ'". iApply HR.
-  Qed.
+  Section sim.
+    #[global] Instance frame_sim p R eₛ eₜ Φ1 Φ2 :
+      (∀ eₛ eₜ, Frame p R (Φ1 eₛ eₜ) (Φ2 eₛ eₜ)) →
+      Frame p R
+        (SIM eₛ ≳ eₜ [[ X ]] {{ Φ1 }})
+        (SIM eₛ ≳ eₜ [[ X ]] {{ Φ2 }}).
+    Proof.
+      rewrite /Frame sim_frame_l.
+      iIntros "%HR Hsim".
+      iApply (sim_mono with "[] Hsim"). iIntros "%eₛ' %eₜ'". iApply HR.
+    Qed.
 
-  #[global] Instance elim_modal_cupd_simv p P eₛ eₜ Φ :
-    ElimModal True p false (|++> P) P
-      (SIM eₛ ≳ eₜ [[ X ]] [[ Φ ]])
-      (SIM eₛ ≳ eₜ [[ X ]] [[ Φ ]]).
-  Proof.
-    rewrite /ElimModal bi.intuitionistically_if_elim.
-    iIntros "_ (HP & Hsim)".
-    iApply cupd_simv. iMod "HP". iModIntro. iApply ("Hsim" with "HP").
-  Qed.
-  #[global] Instance elim_modal_bupd_simv p P eₛ eₜ Φ :
-    ElimModal True p false (|==> P) P
-      (SIM eₛ ≳ eₜ [[ X ]] [[ Φ ]])
-      (SIM eₛ ≳ eₜ [[ X ]] [[ Φ ]]).
-  Proof.
-    rewrite /ElimModal bi.intuitionistically_if_elim.
-    iIntros "_ (HP & Hsim)".
-    iApply bupd_simv. iMod "HP". iModIntro. iApply ("Hsim" with "HP").
-  Qed.
+    #[global] Instance elim_modal_cupd_sim p P eₛ eₜ Φ :
+      ElimModal True p false (|++> P) P
+        (SIM eₛ ≳ eₜ [[ X ]] {{ Φ }})
+        (SIM eₛ ≳ eₜ [[ X ]] {{ Φ }}).
+    Proof.
+      rewrite /ElimModal bi.intuitionistically_if_elim.
+      iIntros "_ (HP & Hsim)".
+      iApply cupd_sim. iMod "HP". iModIntro. iApply ("Hsim" with "HP").
+    Qed.
+    #[global] Instance elim_modal_bupd_sim p P eₛ eₜ Φ :
+      ElimModal True p false (|==> P) P
+        (SIM eₛ ≳ eₜ [[ X ]] {{ Φ }})
+        (SIM eₛ ≳ eₜ [[ X ]] {{ Φ }}).
+    Proof.
+      rewrite /ElimModal bi.intuitionistically_if_elim.
+      iIntros "_ (HP & Hsim)".
+      iApply bupd_sim. iMod "HP". iModIntro. iApply ("Hsim" with "HP").
+    Qed.
 
-  #[global] Instance add_modal_cupd_simv P eₛ eₜ Φ :
-    AddModal (|++> P) P (SIM eₛ ≳ eₜ [[ X ]] [[ Φ ]]).
-  Proof.
-    rewrite /AddModal.
-    iIntros "(HP & Hsim)".
-    iApply cupd_simv. iMod "HP". iApply ("Hsim" with "HP").
-  Qed.
-  #[global] Instance add_modal_bupd_simv P eₛ eₜ Φ :
-    AddModal (|==> P) P (SIM eₛ ≳ eₜ [[ X ]] [[ Φ ]]).
-  Proof.
-    rewrite /AddModal.
-    iIntros "(HP & Hsim)".
-    iApply bupd_simv. iMod "HP". iApply ("Hsim" with "HP").
-  Qed.
+    #[global] Instance add_modal_cupd_sim P eₛ eₜ Φ :
+      AddModal (|++> P) P (SIM eₛ ≳ eₜ [[ X ]] {{ Φ }}).
+    Proof.
+      rewrite /AddModal.
+      iIntros "(HP & Hsim)".
+      iApply cupd_sim. iMod "HP". iApply ("Hsim" with "HP").
+    Qed.
+    #[global] Instance add_modal_bupd_sim P eₛ eₜ Φ :
+      AddModal (|==> P) P (SIM eₛ ≳ eₜ [[ X ]] {{ Φ }}).
+    Proof.
+      rewrite /AddModal.
+      iIntros "(HP & Hsim)".
+      iApply bupd_sim. iMod "HP". iApply ("Hsim" with "HP").
+    Qed.
 
-  Lemma tac_simv_eval eₛ eₛ' eₜ eₜ' Φ Δ :
-    (∀ (eₛ'' := eₛ'), eₛ = eₛ'') →
-    (∀ (eₜ'' := eₜ'), eₜ = eₜ'') →
-    envs_entails Δ (SIM eₛ' ≳ eₜ' [[ X ]] [[ Φ ]]) →
-    envs_entails Δ (SIM eₛ ≳ eₜ [[ X ]] [[ Φ ]]).
-  Proof.
-    intros -> ->. done.
-  Qed.
+    Lemma tac_sim_eval eₛ eₛ' eₜ eₜ' Φ Δ :
+      (∀ (eₛ'' := eₛ'), eₛ = eₛ'') →
+      (∀ (eₜ'' := eₜ'), eₜ = eₜ'') →
+      envs_entails Δ (SIM eₛ' ≳ eₜ' [[ X ]] {{ Φ }}) →
+      envs_entails Δ (SIM eₛ ≳ eₜ [[ X ]] {{ Φ }}).
+    Proof.
+      intros -> ->. done.
+    Qed.
 
-  Lemma tac_simv_strongly_stuck eₛ eₜ Φ Δ :
-    IsStronglyStuck sim_progₛ eₛ →
-    IsStronglyStuck sim_progₜ eₜ →
-    envs_entails Δ (SIM eₛ ≳ eₜ [[ X ]] [[ Φ ]]).
-  Proof.
-    rewrite envs_entails_unseal.
-    iIntros. iApply simv_strongly_stuck; done.
-  Qed.
+    Lemma tac_sim_strongly_stuck eₛ eₜ Φ Δ :
+      IsStronglyStuck sim_progₛ eₛ →
+      IsStronglyStuck sim_progₜ eₜ →
+      envs_entails Δ (SIM eₛ ≳ eₜ [[ X ]] {{ Φ }}).
+    Proof.
+      rewrite envs_entails_unseal.
+      iIntros. iApply sim_strongly_stuck; done.
+    Qed.
 
-  Lemma tac_simv_post eₛ vₛ eₜ vₜ Φ Δ :
-    eₛ = of_val vₛ →
-    eₜ = of_val vₜ →
-    envs_entails Δ (Φ vₛ vₜ) →
-    envs_entails Δ (SIM eₛ ≳ eₜ [[ X ]] [[ Φ ]]).
-  Proof.
-    rewrite envs_entails_unseal => -> -> ->.
-    iIntros. iApply simv_post; done.
-  Qed.
+    Lemma tac_sim_post eₛ eₜ Φ Δ :
+      envs_entails Δ (Φ eₛ eₜ) →
+      envs_entails Δ (SIM eₛ ≳ eₜ [[ X ]] {{ Φ }}).
+    Proof.
+      rewrite envs_entails_unseal => ->.
+      iIntros. iApply sim_post. done.
+    Qed.
 
-  Lemma tac_cupd_simv eₛ eₜ Φ Δ :
-    envs_entails Δ (|++> SIM eₛ ≳ eₜ [[ X ]] [[ Φ ]]) →
-    envs_entails Δ (SIM eₛ ≳ eₜ [[ X ]] [[ Φ ]]).
-  Proof.
-    rewrite envs_entails_unseal => ->.
-    iApply cupd_simv.
-  Qed.
-  Lemma tac_bupd_simv eₛ eₜ Φ Δ :
-    envs_entails Δ (|==> SIM eₛ ≳ eₜ [[ X ]] [[ Φ ]]) →
-    envs_entails Δ (SIM eₛ ≳ eₜ [[ X ]] [[ Φ ]]).
-  Proof.
-    rewrite envs_entails_unseal => ->.
-    iApply bupd_simv.
-  Qed.
+    Lemma tac_cupd_sim eₛ eₜ Φ Δ :
+      envs_entails Δ (|++> SIM eₛ ≳ eₜ [[ X ]] {{ Φ }}) →
+      envs_entails Δ (SIM eₛ ≳ eₜ [[ X ]] {{ Φ }}).
+    Proof.
+      rewrite envs_entails_unseal => ->.
+      iApply cupd_sim.
+    Qed.
+    Lemma tac_bupd_sim eₛ eₜ Φ Δ :
+      envs_entails Δ (|==> SIM eₛ ≳ eₜ [[ X ]] {{ Φ }}) →
+      envs_entails Δ (SIM eₛ ≳ eₜ [[ X ]] {{ Φ }}).
+    Proof.
+      rewrite envs_entails_unseal => ->.
+      iApply bupd_sim.
+    Qed.
 
-  Lemma tac_simv_cupd eₛ eₜ Φ Δ :
-    envs_entails Δ (SIM eₛ ≳ eₜ [[ X ]] [[ λ eₛ eₜ, |++> Φ eₛ eₜ ]]) →
-    envs_entails Δ (SIM eₛ ≳ eₜ [[ X ]] [[ Φ ]]).
-  Proof.
-    rewrite envs_entails_unseal => ->.
-    iApply simv_cupd.
-  Qed.
-  Lemma tac_simv_bupd eₛ eₜ Φ Δ :
-    envs_entails Δ (SIM eₛ ≳ eₜ [[ X ]] [[ λ eₛ eₜ, |==> Φ eₛ eₜ ]]) →
-    envs_entails Δ (SIM eₛ ≳ eₜ [[ X ]] [[ Φ ]]).
-  Proof.
-    rewrite envs_entails_unseal => ->.
-    iApply simv_bupd.
-  Qed.
+    Lemma tac_sim_cupd eₛ eₜ Φ Δ :
+      envs_entails Δ (SIM eₛ ≳ eₜ [[ X ]] {{ λ eₛ eₜ, |++> Φ eₛ eₜ }}) →
+      envs_entails Δ (SIM eₛ ≳ eₜ [[ X ]] {{ Φ }}).
+    Proof.
+      rewrite envs_entails_unseal => ->.
+      iApply sim_cupd.
+    Qed.
+    Lemma tac_sim_bupd eₛ eₜ Φ Δ :
+      envs_entails Δ (SIM eₛ ≳ eₜ [[ X ]] {{ λ eₛ eₜ, |==> Φ eₛ eₜ }}) →
+      envs_entails Δ (SIM eₛ ≳ eₜ [[ X ]] {{ Φ }}).
+    Proof.
+      rewrite envs_entails_unseal => ->.
+      iApply sim_bupd.
+    Qed.
 
-  Lemma tac_simv_bind Kₛ fₛ eₛ Kₜ fₜ eₜ Φ Δ :
-    fₛ = (λ vₛ, Kₛ @@ vₛ) →
-    fₜ = (λ vₜ, Kₜ @@ vₜ) →
-    envs_entails Δ (
-      SIM eₛ ≳ eₜ [[ X ]] [[ λ vₛ vₜ,
-        SIM fₛ (of_val vₛ) ≳ fₜ (of_val vₜ) [[ X ]] [[ Φ ]]
-      ]]
-    ) →
-    envs_entails Δ (
-      SIM Kₛ @@ eₛ ≳ Kₜ @@ eₜ [[ X ]] [[ Φ ]]
-    ).
-  Proof.
-    rewrite envs_entails_unseal -simv_bind => -> -> -> //.
-  Qed.
-  Lemma tac_simv_bindₛ K f eₛ eₜ Φ Δ :
-    f = (λ vₛ, K @@ vₛ) →
-    envs_entails Δ (
-      SIM eₛ ≳ eₜ [[ X ]] [[ λ vₛ vₜ,
-        SIM f (of_val vₛ) ≳ of_val vₜ [[ X ]] [[ Φ ]]
-      ]]
-    ) →
-    envs_entails Δ (
-      SIM K @@ eₛ ≳ eₜ [[ X ]] [[ Φ ]]
-    ).
-  Proof.
-    rewrite envs_entails_unseal -simv_bindₛ => -> -> //.
-  Qed.
-  Lemma tac_simv_bindₜ eₛ K f eₜ Φ Δ :
-    f = (λ eₜ, K @@ eₜ) →
-    envs_entails Δ (
-      SIM eₛ ≳ eₜ [[ X ]] [[ λ vₛ vₜ,
-        SIM of_val vₛ ≳ f (of_val vₜ) [[ X ]] [[ Φ ]]
-      ]]
-    ) →
-    envs_entails Δ (
-      SIM eₛ ≳ K @@ eₜ [[ X ]] [[ Φ ]]
-    ).
-  Proof.
-    rewrite envs_entails_unseal -simv_bindₜ => -> -> //.
-  Qed.
+    Lemma tac_sim_bind Kₛ fₛ eₛ Kₜ fₜ eₜ Φ Δ :
+      fₛ = (λ eₛ, Kₛ @@ eₛ) →
+      fₜ = (λ eₜ, Kₜ @@ eₜ) →
+      envs_entails Δ (
+        SIM eₛ ≳ eₜ [[ X ]] {{ λ eₛ' eₜ',
+          SIM fₛ eₛ' ≳ fₜ eₜ' [[ X ]] {{ Φ }}
+        }}
+      ) →
+      envs_entails Δ (
+        SIM Kₛ @@ eₛ ≳ Kₜ @@ eₜ [[ X ]] {{ Φ }}
+      ).
+    Proof.
+      rewrite envs_entails_unseal -sim_bind => -> -> -> //.
+    Qed.
+    Lemma tac_sim_bindₛ K f eₛ eₜ Φ Δ :
+      f = (λ eₛ, K @@ eₛ) →
+      envs_entails Δ (
+        SIM eₛ ≳ eₜ [[ X ]] {{ λ eₛ' eₜ',
+          SIM f eₛ' ≳ eₜ' [[ X ]] {{ Φ }}
+        }}
+      ) →
+      envs_entails Δ (
+        SIM K @@ eₛ ≳ eₜ [[ X ]] {{ Φ }}
+      ).
+    Proof.
+      rewrite envs_entails_unseal -sim_bindₛ => -> -> //.
+    Qed.
+    Lemma tac_sim_bindₜ eₛ K f eₜ Φ Δ :
+      f = (λ eₜ, K @@ eₜ) →
+      envs_entails Δ (
+        SIM eₛ ≳ eₜ [[ X ]] {{ λ eₛ' eₜ',
+          SIM eₛ' ≳ f eₜ' [[ X ]] {{ Φ }}
+        }}
+      ) →
+      envs_entails Δ (
+        SIM eₛ ≳ K @@ eₜ [[ X ]] {{ Φ }}
+      ).
+    Proof.
+      rewrite envs_entails_unseal -sim_bindₜ => -> -> //.
+    Qed.
 
-  Lemma tac_simv_pure_execₛ ϕ n K eₛ1 eₛ2 eₜ Φ Δ :
-    PureExec sim_progₛ ϕ n eₛ1 eₛ2 →
-    ϕ →
-    envs_entails Δ (SIM K @@ eₛ2 ≳ eₜ [[ X ]] [[ Φ ]]) →
-    envs_entails Δ (SIM K @@ eₛ1 ≳ eₜ [[ X ]] [[ Φ ]]).
-  Proof.
-    pose proof @pure_exec_fill_pure_exec.
-    rewrite envs_entails_unseal => ? ? ->.
-    eapply simv_pure_stepsₛ, rtc_nsteps_2, pure_exec_pure_steps; done.
-  Qed.
-  Lemma tac_simv_pure_execₜ ϕ n eₛ K eₜ1 eₜ2 Φ Δ :
-    PureExec sim_progₜ ϕ n eₜ1 eₜ2 →
-    ϕ →
-    envs_entails Δ (SIM eₛ ≳ K @@ eₜ2 [[ X ]] [[ Φ ]]) →
-    envs_entails Δ (SIM eₛ ≳ K @@ eₜ1 [[ X ]] [[ Φ ]]).
-  Proof.
-    pose proof @pure_exec_fill_pure_exec.
-    rewrite envs_entails_unseal => ? ? ->.
-    eapply simv_pure_stepsₜ, rtc_nsteps_2, pure_exec_pure_steps; done.
-  Qed.
-End sim.
+    Lemma tac_sim_pure_execₛ ϕ n K eₛ1 eₛ2 eₜ Φ Δ :
+      PureExec sim_progₛ ϕ n eₛ1 eₛ2 →
+      ϕ →
+      envs_entails Δ (SIM K @@ eₛ2 ≳ eₜ [[ X ]] {{ Φ }}) →
+      envs_entails Δ (SIM K @@ eₛ1 ≳ eₜ [[ X ]] {{ Φ }}).
+    Proof.
+      pose proof @pure_exec_fill_pure_exec.
+      rewrite envs_entails_unseal => ? ? ->.
+      eapply sim_pure_stepsₛ, rtc_nsteps_2, pure_exec_pure_steps; done.
+    Qed.
+    Lemma tac_sim_pure_execₜ ϕ n eₛ K eₜ1 eₜ2 Φ Δ :
+      PureExec sim_progₜ ϕ n eₜ1 eₜ2 →
+      ϕ →
+      envs_entails Δ (SIM eₛ ≳ K @@ eₜ2 [[ X ]] {{ Φ }}) →
+      envs_entails Δ (SIM eₛ ≳ K @@ eₜ1 [[ X ]] {{ Φ }}).
+    Proof.
+      pose proof @pure_exec_fill_pure_exec.
+      rewrite envs_entails_unseal => ? ? ->.
+      eapply sim_pure_stepsₜ, rtc_nsteps_2, pure_exec_pure_steps; done.
+    Qed.
+  End sim.
 
-Tactic Notation "ectx_is_empty" open_constr(K) :=
+  Section simv.
+    #[global] Instance frame_simv p R eₛ eₜ Φ1 Φ2 :
+      (∀ eₛ eₜ, Frame p R (Φ1 eₛ eₜ) (Φ2 eₛ eₜ)) →
+      Frame p R
+        (SIM eₛ ≳ eₜ [[ X ]] [[ Φ1 ]])
+        (SIM eₛ ≳ eₜ [[ X ]] [[ Φ2 ]]).
+    Proof.
+      rewrite /Frame simv_frame_l.
+      iIntros "%HR Hsim".
+      iApply (simv_mono with "[] Hsim"). iIntros "%eₛ' %eₜ'". iApply HR.
+    Qed.
+
+    #[global] Instance elim_modal_cupd_simv p P eₛ eₜ Φ :
+      ElimModal True p false (|++> P) P
+        (SIM eₛ ≳ eₜ [[ X ]] [[ Φ ]])
+        (SIM eₛ ≳ eₜ [[ X ]] [[ Φ ]]).
+    Proof.
+      rewrite /ElimModal bi.intuitionistically_if_elim.
+      iIntros "_ (HP & Hsim)".
+      iApply cupd_simv. iMod "HP". iModIntro. iApply ("Hsim" with "HP").
+    Qed.
+    #[global] Instance elim_modal_bupd_simv p P eₛ eₜ Φ :
+      ElimModal True p false (|==> P) P
+        (SIM eₛ ≳ eₜ [[ X ]] [[ Φ ]])
+        (SIM eₛ ≳ eₜ [[ X ]] [[ Φ ]]).
+    Proof.
+      rewrite /ElimModal bi.intuitionistically_if_elim.
+      iIntros "_ (HP & Hsim)".
+      iApply bupd_simv. iMod "HP". iModIntro. iApply ("Hsim" with "HP").
+    Qed.
+
+    #[global] Instance add_modal_cupd_simv P eₛ eₜ Φ :
+      AddModal (|++> P) P (SIM eₛ ≳ eₜ [[ X ]] [[ Φ ]]).
+    Proof.
+      rewrite /AddModal.
+      iIntros "(HP & Hsim)".
+      iApply cupd_simv. iMod "HP". iApply ("Hsim" with "HP").
+    Qed.
+    #[global] Instance add_modal_bupd_simv P eₛ eₜ Φ :
+      AddModal (|==> P) P (SIM eₛ ≳ eₜ [[ X ]] [[ Φ ]]).
+    Proof.
+      rewrite /AddModal.
+      iIntros "(HP & Hsim)".
+      iApply bupd_simv. iMod "HP". iApply ("Hsim" with "HP").
+    Qed.
+
+    Lemma tac_simv_eval eₛ eₛ' eₜ eₜ' Φ Δ :
+      (∀ (eₛ'' := eₛ'), eₛ = eₛ'') →
+      (∀ (eₜ'' := eₜ'), eₜ = eₜ'') →
+      envs_entails Δ (SIM eₛ' ≳ eₜ' [[ X ]] [[ Φ ]]) →
+      envs_entails Δ (SIM eₛ ≳ eₜ [[ X ]] [[ Φ ]]).
+    Proof.
+      intros -> ->. done.
+    Qed.
+
+    Lemma tac_simv_strongly_stuck eₛ eₜ Φ Δ :
+      IsStronglyStuck sim_progₛ eₛ →
+      IsStronglyStuck sim_progₜ eₜ →
+      envs_entails Δ (SIM eₛ ≳ eₜ [[ X ]] [[ Φ ]]).
+    Proof.
+      rewrite envs_entails_unseal.
+      iIntros. iApply simv_strongly_stuck; done.
+    Qed.
+
+    Lemma tac_simv_post eₛ vₛ eₜ vₜ Φ Δ :
+      eₛ = of_val vₛ →
+      eₜ = of_val vₜ →
+      envs_entails Δ (Φ vₛ vₜ) →
+      envs_entails Δ (SIM eₛ ≳ eₜ [[ X ]] [[ Φ ]]).
+    Proof.
+      rewrite envs_entails_unseal => -> -> ->.
+      iIntros. iApply simv_post; done.
+    Qed.
+
+    Lemma tac_cupd_simv eₛ eₜ Φ Δ :
+      envs_entails Δ (|++> SIM eₛ ≳ eₜ [[ X ]] [[ Φ ]]) →
+      envs_entails Δ (SIM eₛ ≳ eₜ [[ X ]] [[ Φ ]]).
+    Proof.
+      rewrite envs_entails_unseal => ->.
+      iApply cupd_simv.
+    Qed.
+    Lemma tac_bupd_simv eₛ eₜ Φ Δ :
+      envs_entails Δ (|==> SIM eₛ ≳ eₜ [[ X ]] [[ Φ ]]) →
+      envs_entails Δ (SIM eₛ ≳ eₜ [[ X ]] [[ Φ ]]).
+    Proof.
+      rewrite envs_entails_unseal => ->.
+      iApply bupd_simv.
+    Qed.
+
+    Lemma tac_simv_cupd eₛ eₜ Φ Δ :
+      envs_entails Δ (SIM eₛ ≳ eₜ [[ X ]] [[ λ eₛ eₜ, |++> Φ eₛ eₜ ]]) →
+      envs_entails Δ (SIM eₛ ≳ eₜ [[ X ]] [[ Φ ]]).
+    Proof.
+      rewrite envs_entails_unseal => ->.
+      iApply simv_cupd.
+    Qed.
+    Lemma tac_simv_bupd eₛ eₜ Φ Δ :
+      envs_entails Δ (SIM eₛ ≳ eₜ [[ X ]] [[ λ eₛ eₜ, |==> Φ eₛ eₜ ]]) →
+      envs_entails Δ (SIM eₛ ≳ eₜ [[ X ]] [[ Φ ]]).
+    Proof.
+      rewrite envs_entails_unseal => ->.
+      iApply simv_bupd.
+    Qed.
+
+    Lemma tac_simv_bind Kₛ fₛ eₛ Kₜ fₜ eₜ Φ Δ :
+      fₛ = (λ eₛ, Kₛ @@ eₛ) →
+      fₜ = (λ eₜ, Kₜ @@ eₜ) →
+      envs_entails Δ (
+        SIM eₛ ≳ eₜ [[ X ]] [[ λ vₛ vₜ,
+          SIM fₛ (of_val vₛ) ≳ fₜ (of_val vₜ) [[ X ]] [[ Φ ]]
+        ]]
+      ) →
+      envs_entails Δ (
+        SIM Kₛ @@ eₛ ≳ Kₜ @@ eₜ [[ X ]] [[ Φ ]]
+      ).
+    Proof.
+      rewrite envs_entails_unseal -simv_bind => -> -> -> //.
+    Qed.
+    Lemma tac_simv_bindₛ K f eₛ eₜ Φ Δ :
+      f = (λ eₛ, K @@ eₛ) →
+      envs_entails Δ (
+        SIM eₛ ≳ eₜ [[ X ]] [[ λ vₛ vₜ,
+          SIM f (of_val vₛ) ≳ of_val vₜ [[ X ]] [[ Φ ]]
+        ]]
+      ) →
+      envs_entails Δ (
+        SIM K @@ eₛ ≳ eₜ [[ X ]] [[ Φ ]]
+      ).
+    Proof.
+      rewrite envs_entails_unseal -simv_bindₛ => -> -> //.
+    Qed.
+    Lemma tac_simv_bindₜ eₛ K f eₜ Φ Δ :
+      f = (λ eₜ, K @@ eₜ) →
+      envs_entails Δ (
+        SIM eₛ ≳ eₜ [[ X ]] [[ λ vₛ vₜ,
+          SIM of_val vₛ ≳ f (of_val vₜ) [[ X ]] [[ Φ ]]
+        ]]
+      ) →
+      envs_entails Δ (
+        SIM eₛ ≳ K @@ eₜ [[ X ]] [[ Φ ]]
+      ).
+    Proof.
+      rewrite envs_entails_unseal -simv_bindₜ => -> -> //.
+    Qed.
+
+    Lemma tac_simv_pure_execₛ ϕ n K eₛ1 eₛ2 eₜ Φ Δ :
+      PureExec sim_progₛ ϕ n eₛ1 eₛ2 →
+      ϕ →
+      envs_entails Δ (SIM K @@ eₛ2 ≳ eₜ [[ X ]] [[ Φ ]]) →
+      envs_entails Δ (SIM K @@ eₛ1 ≳ eₜ [[ X ]] [[ Φ ]]).
+    Proof.
+      pose proof @pure_exec_fill_pure_exec.
+      rewrite envs_entails_unseal => ? ? ->.
+      eapply simv_pure_stepsₛ, rtc_nsteps_2, pure_exec_pure_steps; done.
+    Qed.
+    Lemma tac_simv_pure_execₜ ϕ n eₛ K eₜ1 eₜ2 Φ Δ :
+      PureExec sim_progₜ ϕ n eₜ1 eₜ2 →
+      ϕ →
+      envs_entails Δ (SIM eₛ ≳ K @@ eₜ2 [[ X ]] [[ Φ ]]) →
+      envs_entails Δ (SIM eₛ ≳ K @@ eₜ1 [[ X ]] [[ Φ ]]).
+    Proof.
+      pose proof @pure_exec_fill_pure_exec.
+      rewrite envs_entails_unseal => ? ? ->.
+      eapply simv_pure_stepsₜ, rtc_nsteps_2, pure_exec_pure_steps; done.
+    Qed.
+  End simv.
+End sim_state.
+
+#[local] Tactic Notation "expr_is_val" open_constr(e) :=
+  eunify (of_val _) e.
+
+#[local] Tactic Notation "ectx_is_empty" open_constr(K) :=
   let ectx := type of K in
   unshelve unify (empty : ectx) K; [].
 
-Tactic Notation "match_simv" tactic3(tac_succ) tactic3(tac_fail) :=
+Tactic Notation "match_sim_or_simv" tactic3(tac_sim) tactic3(tac_simv) tactic3(tac_fail) :=
   iStartProof;
   lazymatch goal with
+  | |- envs_entails ?Δ (sim ?X ?Φ ?eₛ ?eₜ) =>
+      tac_sim Δ X Φ eₛ eₜ
   | |- envs_entails ?Δ (simv ?X ?Φ ?eₛ ?eₜ) =>
-      tac_succ Δ X Φ eₛ eₜ
+      tac_simv Δ X Φ eₛ eₜ
   | _ =>
       tac_fail ()
   end.
+Tactic Notation "match_sim_or_simv'" tactic3(tac_succ) tactic3(tac_fail) :=
+  match_sim_or_simv
+    ltac:(tac_succ)
+    ltac:(tac_succ)
+    ltac:(tac_fail).
+Tactic Notation "match_sim" tactic3(tac_succ) tactic3(tac_fail) :=
+  match_sim_or_simv
+    ltac:(tac_succ)
+    ltac:(fun _ _ _ _ _ => tac_fail ())
+    ltac:(tac_fail).
+Tactic Notation "match_simv" tactic3(tac_succ) tactic3(tac_fail) :=
+  match_sim_or_simv
+    ltac:(fun _ _ _ _ _ => tac_fail ())
+    ltac:(tac_succ)
+    ltac:(tac_fail).
 
+Tactic Notation "on_sim_or_simv" tactic3(tac_sim) tactic3(tac_simv) :=
+  match_sim_or_simv
+    ltac:(tac_sim)
+    ltac:(tac_simv)
+    ltac:(fun _ => fail "not a 'sim' or a 'simv'").
+Tactic Notation "on_sim_or_simv'" tactic3(tac) :=
+  on_sim_or_simv
+    ltac:(tac)
+    ltac:(tac).
+Tactic Notation "on_sim" tactic3(tac) :=
+  match_sim
+    ltac:(tac)
+    ltac:(fun _ => fail "not a 'sim'").
 Tactic Notation "on_simv" tactic3(tac) :=
-  match_simv ltac:(tac) ltac:(fun _ => fail "not a 'simv'").
+  match_simv
+    ltac:(tac)
+    ltac:(fun _ => fail "not a 'simv'").
 
-Tactic Notation "simv_eval" tactic3(tacₛ) tactic3(tacₜ) :=
-  on_simv ltac:(fun _ _ _ _ _ =>
-    notypeclasses refine (tac_simv_eval _ _ _ _ _ _ _ _ _ _);
-    [ let x := fresh in intros x; tacₛ; unfold x; notypeclasses refine eq_refl
-    | let x := fresh in intros x; tacₜ; unfold x; notypeclasses refine eq_refl
-    | idtac
-    ]
-  ).
-Tactic Notation "simv_eval" tactic3(tac) :=
-  simv_eval ltac:(tac) ltac:(tac).
-Tactic Notation "simv_evalₛ" tactic3(tac) :=
-  simv_eval ltac:(tac) ltac:(idtac).
-Tactic Notation "simv_evalₜ" tactic3(tac) :=
-  simv_eval ltac:(idtac) ltac:(tac).
+Tactic Notation "sim_eval" tactic3(tacₛ) tactic3(tacₜ) :=
+  on_sim_or_simv
+    ltac:(fun _ _ _ _ _ => notypeclasses refine (tac_sim_eval _ _ _ _ _ _ _ _ _ _))
+    ltac:(fun _ _ _ _ _ => notypeclasses refine (tac_simv_eval _ _ _ _ _ _ _ _ _ _));
+  [ let x := fresh in intros x; tacₛ; unfold x; notypeclasses refine eq_refl
+  | let x := fresh in intros x; tacₜ; unfold x; notypeclasses refine eq_refl
+  | idtac
+  ].
+Tactic Notation "sim_eval" tactic3(tac) :=
+  sim_eval ltac:(tac) ltac:(tac).
+Tactic Notation "sim_evalₛ" tactic3(tac) :=
+  sim_eval ltac:(tac) ltac:(idtac).
+Tactic Notation "sim_evalₜ" tactic3(tac) :=
+  sim_eval ltac:(idtac) ltac:(tac).
 
-Ltac simv_simpl :=
-  simv_eval simpl.
-Ltac simv_simplₛ :=
-  simv_evalₛ simpl.
-Ltac simv_simplₜ :=
-  simv_evalₜ simpl.
+Ltac sim_simpl :=
+  sim_eval simpl.
+Ltac sim_simplₛ :=
+  sim_evalₛ simpl.
+Ltac sim_simplₜ :=
+  sim_evalₜ simpl.
 
-Ltac simv_simpl_post :=
-  on_simv ltac:(fun Δ X Φ eₛ eₜ =>
-    let Φ := eval simpl in Φ in
-    change (envs_entails Δ (simv X Φ eₛ eₜ))
-  ).
+Ltac sim_simpl_post :=
+  on_sim_or_simv
+    ltac:(fun Δ X Φ eₛ eₜ =>
+      let Φ := eval simpl in Φ in
+      change (envs_entails Δ (sim X Φ eₛ eₜ))
+    )
+    ltac:(fun Δ X Φ eₛ eₜ =>
+      let Φ := eval simpl in Φ in
+      change (envs_entails Δ (simv X Φ eₛ eₜ))
+    ).
 
-Ltac simv_strongly_stuck :=
-  on_simv ltac:(fun _ _ _ _ _ =>
-    eapply tac_simv_strongly_stuck;
-    [ iSolveTC
-    | iSolveTC
-    ]
-  ).
+Ltac sim_strongly_stuck :=
+  on_sim_or_simv
+    ltac:(fun _ _ _ _ _ => eapply tac_sim_strongly_stuck)
+    ltac:(fun _ _ _ _ _ => eapply tac_simv_strongly_stuck);
+  [ iSolveTC
+  | iSolveTC
+  ].
 
 Ltac cupd_sim :=
-  on_simv ltac:(fun _ _ _ _ _ =>
-    eapply tac_cupd_simv
-  ).
+  on_sim_or_simv
+    ltac:(fun _ _ _ _ _ => eapply tac_cupd_sim)
+    ltac:(fun _ _ _ _ _ => eapply tac_cupd_simv).
 
-Ltac simv_cupd_simple :=
-  on_simv ltac:(fun _ _ _ _ _ =>
-    eapply tac_simv_cupd
-  ).
-Ltac simv_cupd :=
-  on_simv ltac:(fun _ _ Φ _ _ =>
-    first
-    [ assert (∀ P eₛ eₜ, AddModal (|++> P) P (Φ eₛ eₜ)) as _ by iSolveTC
-    | simv_cupd_simple
-    ]
-  ).
+Ltac sim_cupd_simple :=
+  on_sim_or_simv
+    ltac:(fun _ _ _ _ _ => eapply tac_sim_cupd)
+    ltac:(fun _ _ _ _ _ => eapply tac_simv_cupd).
+Ltac sim_cupd :=
+  on_sim_or_simv'
+    ltac:(fun _ _ Φ _ _ =>
+      first
+      [ assert (∀ P eₛ eₜ, AddModal (|++> P) P (Φ eₛ eₜ)) as _ by iSolveTC
+      | sim_cupd_simple
+      ]
+    ).
 
 Ltac bupd_sim :=
-  on_simv ltac:(fun _ _ _ _ _ =>
-    eapply tac_bupd_simv
-  ).
+  on_sim_or_simv
+    ltac:(fun _ _ _ _ _ => eapply tac_bupd_sim)
+    ltac:(fun _ _ _ _ _ => eapply tac_bupd_simv).
 
-Ltac simv_bupd_simple :=
-  on_simv ltac:(fun _ _ _ _ _ =>
-    eapply tac_simv_bupd
-  ).
-Ltac simv_bupd :=
-  on_simv ltac:(fun _ _ Φ _ _ =>
+Ltac sim_bupd_simple :=
+  on_sim_or_simv
+    ltac:(fun _ _ _ _ _ => eapply tac_sim_bupd)
+    ltac:(fun _ _ _ _ _ => eapply tac_simv_bupd).
+Ltac sim_bupd :=
+  on_sim_or_simv' ltac:(fun _ _ Φ _ _ =>
     first
     [ assert (∀ P eₛ eₜ, AddModal (|==> P) P (Φ eₛ eₜ)) as _ by iSolveTC
-    | simv_bupd_simple
+    | sim_bupd_simple
     ]
   ).
 
-Ltac simv_post_simple :=
-  on_simv ltac:(fun _ _ _ _ _ =>
-    eapply tac_simv_post;
-    [ reflexivity
-    | reflexivity
-    | idtac
-    ]
-  ).
-Ltac simv_post :=
-  simv_simpl;
-  simv_cupd;
-  simv_post_simple;
+Ltac sim_post_simple :=
+  on_sim_or_simv
+    ltac:(fun _ _ _ _ _ =>
+      eapply tac_sim_post
+    )
+    ltac:(fun _ _ _ _ _ =>
+      eapply tac_simv_post;
+      [ reflexivity
+      | reflexivity
+      | idtac
+      ]
+    ).
+Ltac sim_post :=
+  sim_simpl;
+  sim_cupd;
+  sim_post_simple;
   try done.
 
-Tactic Notation "simv_finish" "with" tactic3(tac) :=
-  simv_eval (simpl; rewrite ?fill_empty; tac);
-  try simv_post;
+Tactic Notation "sim_finish" "with" tactic3(tac) :=
+  sim_eval (simpl; rewrite ?fill_empty; tac);
+  on_sim_or_simv
+    ltac:(fun _ _ _ eₛ eₜ =>
+      tryif expr_is_val eₛ; expr_is_val eₜ then (
+        sim_post
+      ) else (
+        try solve [sim_post]
+      )
+    )
+    ltac:(fun _ _ _ _ _ =>
+      try sim_post
+    );
   pm_prettify.
-Tactic Notation "simv_finish" :=
-  simv_finish with idtac.
+Tactic Notation "sim_finish" :=
+  sim_finish with idtac.
 
-Tactic Notation "simv_bind_coreₛ" open_constr(K) :=
+Tactic Notation "sim_bind_coreₛ" open_constr(K) :=
   tryif ectx_is_empty K then (
     idtac
   ) else (
-    eapply (tac_simv_bindₛ _ K);
+    on_sim_or_simv
+      ltac:(fun _ _ _ _ _ => eapply (tac_sim_bindₛ _ K))
+      ltac:(fun _ _ _ _ _ => eapply (tac_simv_bindₛ _ K));
     [ simpl; reflexivity
-    | pm_prettify; simv_simpl_post
+    | pm_prettify; sim_simpl_post
     ]
   ).
-Tactic Notation "simv_bind_coreₜ" open_constr(K) :=
+Tactic Notation "sim_bind_coreₜ" open_constr(K) :=
   tryif ectx_is_empty K then (
     idtac
   ) else (
-    eapply (tac_simv_bindₜ _ _ K);
+    on_sim_or_simv
+      ltac:(fun _ _ _ _ _ => eapply (tac_sim_bindₜ _ _ K))
+      ltac:(fun _ _ _ _ _ => eapply (tac_simv_bindₜ _ _ K));
     [ simpl; reflexivity
-    | pm_prettify; simv_simpl_post
+    | pm_prettify; sim_simpl_post
     ]
   ).
-Tactic Notation "simv_bind_core" open_constr(Kₛ) open_constr(Kₜ) :=
+Tactic Notation "sim_bind_core" open_constr(Kₛ) open_constr(Kₜ) :=
   tryif ectx_is_empty Kₛ then (
-    simv_bind_coreₜ Kₜ
+    sim_bind_coreₜ Kₜ
   ) else (
     tryif ectx_is_empty Kₜ then (
-      simv_bind_coreₛ Kₛ
+      sim_bind_coreₛ Kₛ
     ) else (
-      eapply (tac_simv_bind _ Kₛ _ _ Kₜ);
+      on_sim_or_simv
+        ltac:(fun _ _ _ _ _ => eapply (tac_sim_bind _ Kₛ _ _ Kₜ))
+        ltac:(fun _ _ _ _ _ => eapply (tac_simv_bind _ Kₛ _ _ Kₜ));
       [ simpl; reflexivity
       | simpl; reflexivity
-      | pm_prettify; simv_simpl_post
+      | pm_prettify; sim_simpl_post
       ]
     )
   ).
 
-Tactic Notation "simv_pure_coreₛ" open_constr(K) "with" tactic3(tac) :=
-  eapply (tac_simv_pure_execₛ _ _ _ K);
+Tactic Notation "sim_pure_coreₛ" open_constr(K) "with" tactic3(tac) :=
+  on_sim_or_simv
+    ltac:(fun _ _ _ _ _ => eapply (tac_sim_pure_execₛ _ _ _ K))
+    ltac:(fun _ _ _ _ _ => eapply (tac_simv_pure_execₛ _ _ _ K));
   [ iSolveTC
   | try done
-  | simv_finish with tac
+  | sim_finish with tac
   ].
-Tactic Notation "simv_pure_coreₛ" open_constr(K) :=
-  simv_pure_coreₛ K with idtac.
-Tactic Notation "simv_pure_coreₜ" open_constr(K) "with" tactic3(tac) :=
-  eapply (tac_simv_pure_execₜ _ _ _ _ K);
+Tactic Notation "sim_pure_coreₛ" open_constr(K) :=
+  sim_pure_coreₛ K with idtac.
+Tactic Notation "sim_pure_coreₜ" open_constr(K) "with" tactic3(tac) :=
+  on_sim_or_simv
+    ltac:(fun _ _ _ _ _ => eapply (tac_sim_pure_execₜ _ _ _ _ K))
+    ltac:(fun _ _ _ _ _ => eapply (tac_simv_pure_execₜ _ _ _ _ K));
   [ iSolveTC
   | try done
-  | simv_finish with tac
+  | sim_finish with tac
   ].
-Tactic Notation "simv_pure_coreₜ" open_constr(K) :=
-  simv_pure_coreₜ K with idtac.
+Tactic Notation "sim_pure_coreₜ" open_constr(K) :=
+  sim_pure_coreₜ K with idtac.
