theories/tmc/properties.v
@@ -1,0 +1,146 @@
+From simuliris Require Import
+  prelude.
+From simuliris.common Require Import
+  tactics.
+From simuliris.language Require Export
+  well_formed.
+From simuliris.language Require Import
+  notations.
+From simuliris.tmc Require Export
+  definition.
+
+Lemma tmc_dir_refl ξ e :
+  tmc_dir ξ e e.
+Proof.
+  induction e; eauto with tmc.
+Qed.
+#[export] Hint Resolve tmc_dir_refl : tmc.
+
+Lemma tmc_subst ξ :
+  ( ∀ eₛ eₜ,
+    tmc_dir ξ eₛ eₜ →
+    ∀ eₛ' eₜ' ς,
+    eₛ' = eₛ.[ς] →
+    eₜ' = eₜ.[ς] →
+    tmc_dir ξ eₛ' eₜ'
+  ) ∧ (
+    ∀ dst idx eₛ eₜ,
+    tmc_dps ξ dst idx eₛ eₜ →
+    ∀ dst' idx' eₛ' eₜ' ς,
+    dst' = dst.[ς] →
+    idx' = idx.[ς] →
+    eₛ' = eₛ.[ς] →
+    eₜ' = eₜ.[ς] →
+    tmc_dps ξ dst' idx' eₛ' eₜ'
+  ).
+Proof.
+  apply tmc_ind; solve
+  [ intros; simplify; eauto with tmc
+  | intros * ? ? ? IHdps **; simplify;
+    econstructor; try naive_solver; try eapply IHdps with (up ς); autosubst
+  ].
+Qed.
+Lemma tmc_dir_subst ξ ς eₛ eₛ' eₜ eₜ' :
+  tmc_dir ξ eₛ eₜ →
+  eₛ' = eₛ.[ς] →
+  eₜ' = eₜ.[ς] →
+  tmc_dir ξ eₛ' eₜ'.
+Proof.
+  eauto using (proj1 (tmc_subst ξ)).
+Qed.
+Lemma tmc_dps_subst ξ ς dst dst' idx idx' eₛ eₛ' eₜ eₜ' :
+  tmc_dps ξ dst idx eₛ eₜ →
+  dst' = dst.[ς] →
+  idx' = idx.[ς] →
+  eₛ' = eₛ.[ς] →
+  eₜ' = eₜ.[ς] →
+  tmc_dps ξ dst' idx' eₛ' eₜ'.
+Proof.
+  eauto using (proj2 (tmc_subst ξ)).
+Qed.
+
+Section well_formed.
+  Context {progₛ progₜ} (tmc : tmc progₛ progₜ).
+
+  Lemma expr_well_formed_tmc :
+    ( ∀ eₛ eₜ,
+      tmc_dir tmc.(tmc_ξ) eₛ eₜ →
+      ∀ lvl,
+      expr_well_formed progₛ lvl eₛ →
+      expr_well_formed progₜ lvl eₜ
+    ) ∧ (
+      ∀ dst idx eₛ eₜ,
+      tmc_dps tmc.(tmc_ξ) dst idx eₛ eₜ →
+      ∀ lvl,
+      expr_well_formed progₜ lvl dst →
+      expr_well_formed progₜ lvl idx →
+      expr_well_formed progₛ lvl eₛ →
+      expr_well_formed progₜ lvl eₜ
+    ).
+  Proof.
+    apply tmc_ind; try naive_solver.
+    - intros []; try done. intros lvl Hfuncₛ.
+      rewrite /= tmc.(tmc_dom). apply elem_of_union_l. done.
+    - intros * Hdir1 IH1 Hdps2 IH2 lvl (Hwf1 & Hwf2).
+      simpl. split_and!; try naive_solver lia.
+      apply IH2; try naive_solver lia. apply expr_well_formed_lift1. done.
+    - intros * Hdir2 IH2 Hdps1 IH1 lvl (Hwf1 & Hwf2).
+      simpl. split_and!; try naive_solver lia.
+      apply IH1; try naive_solver lia. apply expr_well_formed_lift1. done.
+    - intros * Hdir1 IH1 Hdps2 IH2 lvl Hdst_wf Hidx_wf (Hwf1 & Hwf2).
+      split; first auto. apply IH2; try done; apply expr_well_formed_lift1; done.
+    - intros * Hξ Hdir IH -> lvl Hdst_wf Hidx_wf (Hfuncₛ%lookup_lookup_total_dom & Hwf).
+      eapply (tmc.(tmc_dpss)) in Hfuncₛ as (eₜ' & Hfunc_dpsₜ & ?); last done.
+      simpl. split_and!; try naive_solver lia.
+      + eapply elem_of_dom_2. done.
+      + apply expr_well_formed_lift1. done.
+      + apply expr_well_formed_lift1. done.
+    - intros * Hdir1 IH1 Hdps2 IH2 -> lvl Hdst_wf Hidx_wf (Hwf1 & Hwf2).
+      simpl. split_and!; try naive_solver lia.
+      + apply expr_well_formed_lift1. done.
+      + apply expr_well_formed_lift1. done.
+      + apply (expr_well_formed_le _ (S (S lvl))); first lia.
+        apply expr_well_formed_lift1, IH2; try naive_solver lia.
+        apply expr_well_formed_lift1. done.
+    - intros * Hdir2 IH2 Hdps1 IH1 -> lvl Hdst_wf Hidx_wf (Hwf1 & Hwf2).
+      simpl. split_and!; try naive_solver lia.
+      + apply expr_well_formed_lift1. done.
+      + apply expr_well_formed_lift1. done.
+      + apply (expr_well_formed_le _ (S (S lvl))); first lia.
+        apply expr_well_formed_lift1, IH1; try naive_solver lia.
+        apply expr_well_formed_lift1. done.
+  Qed.
+  Lemma expr_well_formed_tmc_dir lvl eₛ eₜ :
+    tmc_dir tmc.(tmc_ξ) eₛ eₜ →
+    expr_well_formed progₛ lvl eₛ →
+    expr_well_formed progₜ lvl eₜ.
+  Proof.
+    eauto using (proj1 (expr_well_formed_tmc)).
+  Qed.
+  Lemma expr_well_formed_tmc_dps lvl dst idx eₛ eₜ :
+    tmc_dps tmc.(tmc_ξ) dst idx eₛ eₜ →
+    expr_well_formed progₜ lvl dst →
+    expr_well_formed progₜ lvl idx →
+    expr_well_formed progₛ lvl eₛ →
+    expr_well_formed progₜ lvl eₜ.
+  Proof.
+    eauto using (proj2 (expr_well_formed_tmc)).
+  Qed.
+
+  Lemma program_well_formed_tmc :
+    program_well_formed progₛ →
+    program_well_formed progₜ.
+  Proof.
+    rewrite /program_well_formed !map_Forall_lookup => Hwf func eₜ Hfuncₜ.
+    apply elem_of_dom_2 in Hfuncₜ as Hfuncₜ'. rewrite tmc.(tmc_dom) elem_of_union in Hfuncₜ'.
+    destruct Hfuncₜ' as [Hfuncₛ%lookup_lookup_total_dom | (func_dir & Hξ)%elem_of_map_img].
+    - edestruct tmc.(tmc_dirs) as (_eₜ & Hdir & Heq); first done.
+      eapply expr_well_formed_tmc_dir; last naive_solver.
+      rewrite Heq in Hfuncₜ. naive_solver.
+    - pose proof Hξ as Hfunc_dirₛ%elem_of_dom_2%(tmc.(tmc_ξ_dom))%lookup_lookup_total_dom.
+      edestruct tmc.(tmc_dpss) as (eₜ' & Hdps & Heq); [done.. |].
+      rewrite Hfuncₜ in Heq. injection Heq as ->.
+      repeat constructor. eapply expr_well_formed_tmc_dps; [naive_solver.. |].
+      apply (expr_well_formed_le _ 1); naive_solver lia.
+  Qed.
+End well_formed.
