theories/tmc/sim/proofmode.v
@@ -13,7 +13,7 @@ From simuliris.tmc Require Export
 From simuliris.tmc Require Import
   sim.notations.
 
-Section sim.
+Section sim_GS.
   Context `{sim_programs : !SimPrograms ectx_language ectx_language}.
   Context `{sim_GS : !SimGS Σ}.
   Implicit Types constr : constructor.
@@ -22,9 +22,8 @@ Section sim.
   Implicit Types v vₜ vₛ : val.
   Implicit Types e eₜ eₛ : expr.
   Implicit Types K Kₜ Kₛ : ectx.
-  Implicit Types Φ : val → val → iProp Σ.
 
-  Lemma tac_simv_heap_bij_insert id1 p1 id2 lₛ lₜ P Δ :
+  Lemma tac_sim_heap_bij_insert id1 p1 id2 lₛ lₜ P Δ :
     (∀ Q, AddModal (|++> Q) Q P) →
     envs_lookup id1 Δ = Some (p1, lₛ ⋈ lₜ)%I →
     match envs_replace id1 p1 true (Esnoc Enil id2 (lₛ ≈ lₜ)) Δ with
@@ -45,212 +44,357 @@ Section sim.
 
   Context (X : sim_protocol Σ).
 
-  Lemma tac_simv_constr_detₛ id0 id1 id2 K constr v1 v2 e Φ Δ :
-    ( ∀ l,
-      match
-        envs_app false (Esnoc (Esnoc (Esnoc Enil
-          id2 ((l +ₗ 2) ↦ₛ v2))
-          id1 ((l +ₗ 1) ↦ₛ v1))
-          id0 ((l +ₗ 0) ↦ₛ constr)
-        ) Δ
-      with
+  Section sim.
+    Implicit Types Φ : expr → expr → iProp Σ.
+
+    Lemma tac_sim_constr_detₛ id0 id1 id2 K constr v1 v2 e Φ Δ :
+      ( ∀ l,
+        match
+          envs_app false (Esnoc (Esnoc (Esnoc Enil
+            id2 ((l +ₗ 2) ↦ₛ v2))
+            id1 ((l +ₗ 1) ↦ₛ v1))
+            id0 ((l +ₗ 0) ↦ₛ constr)
+          ) Δ
+        with
+        | None =>
+            False
+        | Some Δ' =>
+            envs_entails Δ' (SIM K @@ #l ≳ e [[ X ]] {{ Φ }})
+        end
+      ) →
+      envs_entails Δ (SIM K @@ &&constr v1 v2 ≳ e [[ X ]] {{ Φ }}).
+    Proof.
+      rewrite envs_entails_unseal => Hsim.
+      rewrite -sim_bindₛ -sim_constr_detₛ. setoid_rewrite <- sim_bind_invₛ.
+      apply bi.forall_intro => l. specialize (Hsim l).
+      destruct (envs_app _ _ _) as [Δ' |] eqn:HΔ'; last done.
+      rewrite envs_app_sound // /= right_id Hsim.
+      iIntros "H Hl0 Hl1 Hl2". iApply ("H" with "[$Hl0 $Hl1 $Hl2]").
+    Qed.
+    Lemma tac_sim_constr_detₜ id0 id1 id2 e K constr v1 v2 Φ Δ :
+      ( ∀ l,
+        match
+          envs_app false (Esnoc (Esnoc (Esnoc Enil
+            id2 ((l +ₗ 2) ↦ₜ v2))
+            id1 ((l +ₗ 1) ↦ₜ v1))
+            id0 ((l +ₗ 0) ↦ₜ constr)
+          ) Δ
+        with
+        | None =>
+            False
+        | Some Δ' =>
+            envs_entails Δ' (SIM e ≳ K @@ #l [[ X ]] {{ Φ }})
+        end
+      ) →
+      envs_entails Δ (SIM e ≳ K @@ &&constr v1 v2 [[ X ]] {{ Φ }}).
+    Proof.
+      rewrite envs_entails_unseal => Hsim.
+      rewrite -sim_bindₜ -sim_constr_detₜ.
+      apply bi.forall_intro => l. specialize (Hsim l).
+      destruct (envs_app _ _ _) as [Δ' |] eqn:HΔ'; last done.
+      rewrite envs_app_sound // /= right_id Hsim sim_bind_invₜ.
+      iIntros "H Hl0 Hl1 Hl2". iApply ("H" with "[$Hl0 $Hl1 $Hl2]").
+    Qed.
+    Lemma tac_sim_constr_det id constr Kₛ vₛ1 vₛ2 Kₜ vₜ1 vₜ2 Φ Δ :
+      envs_entails Δ (vₛ1 ≈ vₜ1) →
+      envs_entails Δ (vₛ2 ≈ vₜ2) →
+      ( ∀ lₛ lₜ,
+        match envs_app true (Esnoc Enil id (Loc lₛ ≈ Loc lₜ)) Δ with
+        | None =>
+            False
+        | Some Δ' =>
+            envs_entails Δ' (SIM Kₛ @@ #lₛ ≳ Kₜ @@ #lₜ [[ X ]] {{ Φ }})
+        end
+      ) →
+      envs_entails Δ (SIM Kₛ @@ &&constr vₛ1 vₛ2 ≳ Kₜ @@ &&constr vₜ1 vₜ2 [[ X ]] {{ Φ }}).
+    Proof.
+      rewrite envs_entails_unseal => Hv1 Hv2 Hsim.
+      iIntros "HΔ".
+      iDestruct (Hv1 with "HΔ") as "#Hv1".
+      iDestruct (Hv2 with "HΔ") as "#Hv2".
+      iApply sim_bind.
+      iApply (sim_constr_det with "Hv1 Hv2"). iIntros "%lₛ %lₜ #Hl !>".
+      specialize (Hsim lₛ lₜ). destruct (envs_app _ _ _) as [Δ' |] eqn:HΔ'; last done.
+      iApply Hsim.
+      iApply (envs_app_sound with "HΔ"); first done. simpl. auto with iFrame.
+    Qed.
+
+    Lemma tac_sim_constrₛ1 K constr e1 e2 e Φ Δ :
+      envs_entails Δ (SIM K @@ let: e1 in let: e2.[ren (+1)] in &&constr $1 $0 ≳ e [[ X ]] {{ Φ }}) →
+      envs_entails Δ (SIM K @@ &constr e1 e2 ≳ e [[ X ]] {{ Φ }}).
+    Proof.
+      rewrite envs_entails_unseal sim_bind_invₛ sim_constrₛ1 sim_bindₛ //.
+    Qed.
+    Lemma tac_sim_constrₛ2 K constr e1 e2 e Φ Δ :
+      envs_entails Δ (SIM K @@ let: e2 in let: e1.[ren (+1)] in &&constr $0 $1 ≳ e [[ X ]] {{ Φ }}) →
+      envs_entails Δ (SIM K @@ &constr e1 e2 ≳ e [[ X ]] {{ Φ }}).
+    Proof.
+      rewrite envs_entails_unseal sim_bind_invₛ sim_constrₛ2 sim_bindₛ //.
+    Qed.
+    Lemma tac_sim_constrₜ e K constr e1 e2 Φ Δ :
+      envs_entails Δ (SIM e ≳ K @@ let: e1 in let: e2.[ren (+1)] in &&constr $1 $0 [[ X ]] {{ Φ }}) →
+      envs_entails Δ (SIM e ≳ K @@ let: e2 in let: e1.[ren (+1)] in &&constr $0 $1 [[ X ]] {{ Φ }}) →
+      envs_entails Δ (SIM e ≳ K @@ &constr e1 e2 [[ X ]] {{ Φ }}).
+    Proof.
+      rewrite envs_entails_unseal => Hsim1 Hsim2.
+      rewrite -sim_bindₜ -sim_constrₜ -!sim_bind_invₜ.
+      apply bi.and_intro; done.
+    Qed.
+
+    Lemma tac_sim_loadₛ id p K l idx v e Φ Δ :
+      envs_lookup id Δ = Some (p, (l +ₗ idx) ↦ₛ v)%I →
+      envs_entails Δ (SIM K @@ #v ≳ e [[ X ]] {{ Φ }}) →
+      envs_entails Δ (SIM K @@ ![idx] l ≳ e [[ X ]] {{ Φ }}).
+    Proof.
+      rewrite envs_entails_unseal => Hlookup Hsim.
+      rewrite envs_lookup_split // -sim_bindₛ Hsim.
+      destruct p; simpl;
+        [iIntros "(#Hl & Hsim)" | iIntros "(Hl & Hsim)"];
+        iApply (sim_loadₛ with "Hl"); iIntros;
+        iApply sim_bind_invₛ;
+        iApply ("Hsim" with "[$]").
+    Qed.
+    Lemma tac_sim_loadₜ id p e K l idx v Φ Δ :
+      envs_lookup id Δ = Some (p, (l +ₗ idx) ↦ₜ v)%I →
+      envs_entails Δ (SIM e ≳ K @@ #v [[ X ]] {{ Φ }}) →
+      envs_entails Δ (SIM e ≳ K @@ ![idx] l [[ X ]] {{ Φ }}).
+    Proof.
+      rewrite envs_entails_unseal => Hlookup Hsim.
+      rewrite envs_lookup_split // -sim_bindₜ Hsim.
+      destruct p; simpl;
+        [iIntros "(#Hl & Hsim)" | iIntros "(Hl & Hsim)"];
+        iApply (sim_loadₜ with "Hl"); iIntros;
+        iApply sim_bind_invₜ;
+        iApply ("Hsim" with "[$]").
+    Qed.
+    Lemma tac_sim_load id Kₛ lₛ idxₛ Kₜ lₜ idxₜ Φ Δ :
+      envs_entails Δ (Loc lₛ ≈ Loc lₜ) →
+      envs_entails Δ (Index idxₛ ≈ Index idxₜ) →
+      ( ∀ vₛ vₜ,
+        match envs_app true (Esnoc Enil id (vₛ ≈ vₜ)) Δ with
+        | None =>
+            False
+        | Some Δ' =>
+            envs_entails Δ' (SIM Kₛ @@ #vₛ ≳ Kₜ @@ #vₜ [[ X ]] {{ Φ }})
+        end
+      ) →
+      envs_entails Δ (SIM Kₛ @@ ![idxₛ] lₛ ≳ Kₜ @@ ![idxₜ] lₜ [[ X ]] {{ Φ }}).
+    Proof.
+      rewrite envs_entails_unseal => Hl Hidx Hsim.
+      iIntros "HΔ".
+      iDestruct (Hl with "HΔ") as "#Hl".
+      iDestruct (Hidx with "HΔ") as "#Hidx".
+      iApply sim_bind.
+      iApply (sim_load with "Hl Hidx"). iIntros "%vₛ %vₜ #Hv".
+      specialize (Hsim vₛ vₜ). destruct (envs_app _ _ _) as [Δ' |] eqn:HΔ'; last done.
+      iApply sim_bind_inv. iApply Hsim.
+      iApply (envs_app_singleton_sound with "[HΔ] [Hv]"); naive_solver.
+    Qed.
+
+    Lemma tac_sim_storeₛ id p K l idx v w e Φ Δ :
+      envs_lookup id Δ = Some (p, (l +ₗ idx) ↦ₛ w)%I →
+      match envs_replace id p false (Esnoc Enil id ((l +ₗ idx) ↦ₛ v)) Δ with
       | None =>
           False
       | Some Δ' =>
-          envs_entails Δ' (SIM K @@ #l ≳ e [[ X ]] [[ Φ ]])
-      end
-    ) →
-    envs_entails Δ (SIM K @@ &&constr v1 v2 ≳ e [[ X ]] [[ Φ ]]).
-  Proof.
-    rewrite definition.simv_unseal /definition.simv_def.
-    rewrite envs_entails_unseal => Hsim.
-    rewrite -sim_bindₛ -sim_constr_detₛ. setoid_rewrite <- sim_bind_invₛ.
-    apply bi.forall_intro => l. specialize (Hsim l).
-    destruct (envs_app _ _ _) as [Δ' |] eqn:HΔ'; last done.
-    rewrite envs_app_sound // /= right_id Hsim.
-    iIntros "H Hl0 Hl1 Hl2". iApply ("H" with "[$Hl0 $Hl1 $Hl2]").
-  Qed.
-  Lemma tac_simv_constr_detₜ id0 id1 id2 e K constr v1 v2 Φ Δ :
-    ( ∀ l,
-      match
-        envs_app false (Esnoc (Esnoc (Esnoc Enil
-          id2 ((l +ₗ 2) ↦ₜ v2))
-          id1 ((l +ₗ 1) ↦ₜ v1))
-          id0 ((l +ₗ 0) ↦ₜ constr)
-        ) Δ
-      with
+          envs_entails Δ' (SIM K @@ #() ≳ e [[ X ]] {{ Φ }})
+      end →
+      envs_entails Δ (SIM K @@ #l <-[idx]- v ≳ e [[ X ]] {{ Φ }}).
+    Proof.
+      rewrite envs_entails_unseal => Hlookup Hsim.
+      destruct (envs_replace _ _ _ _) as [Δ' |] eqn:HΔ'; last done.
+      rewrite envs_replace_singleton_sound // Hsim.
+      rewrite bi.intuitionistically_if_elim /=.
+      rewrite sim_bind_invₛ -sim_bindₛ. apply bi.wand_elim_l', sim_storeₛ.
+    Qed.
+    Lemma tac_sim_storeₜ id p e K l idx v w Φ Δ :
+      envs_lookup id Δ = Some (p, (l +ₗ idx) ↦ₜ w)%I →
+      match envs_replace id p false (Esnoc Enil id ((l +ₗ idx) ↦ₜ v)) Δ with
       | None =>
           False
       | Some Δ' =>
-          envs_entails Δ' (SIM e ≳ K @@ #l [[ X ]] [[ Φ ]])
-      end
-    ) →
-    envs_entails Δ (SIM e ≳ K @@ &&constr v1 v2 [[ X ]] [[ Φ ]]).
-  Proof.
-    rewrite definition.simv_unseal /definition.simv_def.
-    rewrite envs_entails_unseal => Hsim.
-    rewrite -sim_bindₜ -sim_constr_detₜ.
-    apply bi.forall_intro => l. specialize (Hsim l).
-    destruct (envs_app _ _ _) as [Δ' |] eqn:HΔ'; last done.
-    rewrite envs_app_sound // /= right_id Hsim sim_bind_invₜ.
-    iIntros "H Hl0 Hl1 Hl2". iApply ("H" with "[$Hl0 $Hl1 $Hl2]").
-  Qed.
-  Lemma tac_simv_constr_det id constr Kₛ vₛ1 vₛ2 Kₜ vₜ1 vₜ2 Φ Δ :
-    envs_entails Δ (vₛ1 ≈ vₜ1) →
-    envs_entails Δ (vₛ2 ≈ vₜ2) →
-    ( ∀ lₛ lₜ,
-      match envs_app true (Esnoc Enil id (Loc lₛ ≈ Loc lₜ)) Δ with
+          envs_entails Δ' (SIM e ≳ K @@ #() [[ X ]] {{ Φ }})
+      end →
+      envs_entails Δ (SIM e ≳ K @@ #l <-[idx]- v [[ X ]] {{ Φ }}).
+    Proof.
+      rewrite envs_entails_unseal => Hlookup Hsim.
+      destruct (envs_replace _ _ _ _) as [Δ' |] eqn:HΔ'; last done.
+      rewrite envs_replace_singleton_sound // Hsim.
+      rewrite bi.intuitionistically_if_elim /=.
+      rewrite sim_bind_invₜ -sim_bindₜ. apply bi.wand_elim_l', sim_storeₜ.
+    Qed.
+    Lemma tac_sim_store Kₛ vₛ1 vₛ2 vₛ3 Kₜ vₜ1 vₜ2 vₜ3 Φ Δ :
+      envs_entails Δ (vₛ1 ≈ vₜ1) →
+      envs_entails Δ (vₛ2 ≈ vₜ2) →
+      envs_entails Δ (vₛ3 ≈ vₜ3) →
+      envs_entails Δ (SIM Kₛ @@ #() ≳ Kₜ @@ #() [[ X ]] {{ Φ }}) →
+      envs_entails Δ (SIM Kₛ @@ vₛ1 <-[vₛ2]- vₛ3 ≳ Kₜ @@ vₜ1 <-[vₜ2]- vₜ3 [[ X ]] {{ Φ }}).
+    Proof.
+      rewrite envs_entails_unseal => Hv1 Hv2 Hv3 Hsim.
+      iIntros "HΔ".
+      iDestruct (Hv1 with "HΔ") as "#Hv1".
+      iDestruct (Hv2 with "HΔ") as "#Hv2".
+      iDestruct (Hv3 with "HΔ") as "#Hv3".
+      iApply sim_bind. iApply (sim_store with "Hv1 Hv2 Hv3"). iApply (Hsim with "HΔ").
+    Qed.
+  End sim.
+
+  Section simv.
+    Implicit Types Φ : val → val → iProp Σ.
+
+    Lemma tac_simv_constr_detₛ id0 id1 id2 K constr v1 v2 e Φ Δ :
+      ( ∀ l,
+        match
+          envs_app false (Esnoc (Esnoc (Esnoc Enil
+            id2 ((l +ₗ 2) ↦ₛ v2))
+            id1 ((l +ₗ 1) ↦ₛ v1))
+            id0 ((l +ₗ 0) ↦ₛ constr)
+          ) Δ
+        with
+        | None =>
+            False
+        | Some Δ' =>
+            envs_entails Δ' (SIM K @@ #l ≳ e [[ X ]] [[ Φ ]])
+        end
+      ) →
+      envs_entails Δ (SIM K @@ &&constr v1 v2 ≳ e [[ X ]] [[ Φ ]]).
+    Proof.
+      rewrite definition.simv_unseal /definition.simv_def.
+      apply tac_sim_constr_detₛ.
+    Qed.
+    Lemma tac_simv_constr_detₜ id0 id1 id2 e K constr v1 v2 Φ Δ :
+      ( ∀ l,
+        match
+          envs_app false (Esnoc (Esnoc (Esnoc Enil
+            id2 ((l +ₗ 2) ↦ₜ v2))
+            id1 ((l +ₗ 1) ↦ₜ v1))
+            id0 ((l +ₗ 0) ↦ₜ constr)
+          ) Δ
+        with
+        | None =>
+            False
+        | Some Δ' =>
+            envs_entails Δ' (SIM e ≳ K @@ #l [[ X ]] [[ Φ ]])
+        end
+      ) →
+      envs_entails Δ (SIM e ≳ K @@ &&constr v1 v2 [[ X ]] [[ Φ ]]).
+    Proof.
+      rewrite definition.simv_unseal /definition.simv_def.
+      apply tac_sim_constr_detₜ.
+    Qed.
+    Lemma tac_simv_constr_det id constr Kₛ vₛ1 vₛ2 Kₜ vₜ1 vₜ2 Φ Δ :
+      envs_entails Δ (vₛ1 ≈ vₜ1) →
+      envs_entails Δ (vₛ2 ≈ vₜ2) →
+      ( ∀ lₛ lₜ,
+        match envs_app true (Esnoc Enil id (Loc lₛ ≈ Loc lₜ)) Δ with
+        | None =>
+            False
+        | Some Δ' =>
+            envs_entails Δ' (SIM Kₛ @@ #lₛ ≳ Kₜ @@ #lₜ [[ X ]] [[ Φ ]])
+        end
+      ) →
+      envs_entails Δ (SIM Kₛ @@ &&constr vₛ1 vₛ2 ≳ Kₜ @@ &&constr vₜ1 vₜ2 [[ X ]] [[ Φ ]]).
+    Proof.
+      rewrite definition.simv_unseal /definition.simv_def.
+      apply tac_sim_constr_det.
+    Qed.
+
+    Lemma tac_simv_constrₛ1 K constr e1 e2 e Φ Δ :
+      envs_entails Δ (SIM K @@ let: e1 in let: e2.[ren (+1)] in &&constr $1 $0 ≳ e [[ X ]] [[ Φ ]]) →
+      envs_entails Δ (SIM K @@ &constr e1 e2 ≳ e [[ X ]] [[ Φ ]]).
+    Proof.
+      rewrite definition.simv_unseal /definition.simv_def.
+      apply tac_sim_constrₛ1.
+    Qed.
+    Lemma tac_simv_constrₛ2 K constr e1 e2 e Φ Δ :
+      envs_entails Δ (SIM K @@ let: e2 in let: e1.[ren (+1)] in &&constr $0 $1 ≳ e [[ X ]] [[ Φ ]]) →
+      envs_entails Δ (SIM K @@ &constr e1 e2 ≳ e [[ X ]] [[ Φ ]]).
+    Proof.
+      rewrite definition.simv_unseal /definition.simv_def.
+      apply tac_sim_constrₛ2.
+    Qed.
+    Lemma tac_simv_constrₜ e K constr e1 e2 Φ Δ :
+      envs_entails Δ (SIM e ≳ K @@ let: e1 in let: e2.[ren (+1)] in &&constr $1 $0 [[ X ]] [[ Φ ]]) →
+      envs_entails Δ (SIM e ≳ K @@ let: e2 in let: e1.[ren (+1)] in &&constr $0 $1 [[ X ]] [[ Φ ]]) →
+      envs_entails Δ (SIM e ≳ K @@ &constr e1 e2 [[ X ]] [[ Φ ]]).
+    Proof.
+      rewrite definition.simv_unseal /definition.simv_def.
+      apply tac_sim_constrₜ.
+    Qed.
+
+    Lemma tac_simv_loadₛ id p K l idx v e Φ Δ :
+      envs_lookup id Δ = Some (p, (l +ₗ idx) ↦ₛ v)%I →
+      envs_entails Δ (SIM K @@ #v ≳ e [[ X ]] [[ Φ ]]) →
+      envs_entails Δ (SIM K @@ ![idx] l ≳ e [[ X ]] [[ Φ ]]).
+    Proof.
+      rewrite definition.simv_unseal /definition.simv_def.
+      apply tac_sim_loadₛ.
+    Qed.
+    Lemma tac_simv_loadₜ id p e K l idx v Φ Δ :
+      envs_lookup id Δ = Some (p, (l +ₗ idx) ↦ₜ v)%I →
+      envs_entails Δ (SIM e ≳ K @@ #v [[ X ]] [[ Φ ]]) →
+      envs_entails Δ (SIM e ≳ K @@ ![idx] l [[ X ]] [[ Φ ]]).
+    Proof.
+      rewrite definition.simv_unseal /definition.simv_def.
+      apply tac_sim_loadₜ.
+    Qed.
+    Lemma tac_simv_load id Kₛ lₛ idxₛ Kₜ lₜ idxₜ Φ Δ :
+      envs_entails Δ (Loc lₛ ≈ Loc lₜ) →
+      envs_entails Δ (Index idxₛ ≈ Index idxₜ) →
+      ( ∀ vₛ vₜ,
+        match envs_app true (Esnoc Enil id (vₛ ≈ vₜ)) Δ with
+        | None =>
+            False
+        | Some Δ' =>
+            envs_entails Δ' (SIM Kₛ @@ #vₛ ≳ Kₜ @@ #vₜ [[ X ]] [[ Φ ]])
+        end
+      ) →
+      envs_entails Δ (SIM Kₛ @@ ![idxₛ] lₛ ≳ Kₜ @@ ![idxₜ] lₜ [[ X ]] [[ Φ ]]).
+    Proof.
+      rewrite definition.simv_unseal /definition.simv_def.
+      apply tac_sim_load.
+    Qed.
+
+    Lemma tac_simv_storeₛ id p K l idx v w e Φ Δ :
+      envs_lookup id Δ = Some (p, (l +ₗ idx) ↦ₛ w)%I →
+      match envs_replace id p false (Esnoc Enil id ((l +ₗ idx) ↦ₛ v)) Δ with
       | None =>
           False
       | Some Δ' =>
-          envs_entails Δ' (SIM Kₛ @@ #lₛ ≳ Kₜ @@ #lₜ [[ X ]] [[ Φ ]])
-      end
-    ) →
-    envs_entails Δ (SIM Kₛ @@ &&constr vₛ1 vₛ2 ≳ Kₜ @@ &&constr vₜ1 vₜ2 [[ X ]] [[ Φ ]]).
-  Proof.
-    rewrite definition.simv_unseal /definition.simv_def.
-    rewrite envs_entails_unseal => Hv1 Hv2 Hsim.
-    iIntros "HΔ".
-    iDestruct (Hv1 with "HΔ") as "#Hv1".
-    iDestruct (Hv2 with "HΔ") as "#Hv2".
-    iApply sim_bind.
-    iApply (sim_constr_det with "Hv1 Hv2"). iIntros "%lₛ %lₜ #Hl !>".
-    specialize (Hsim lₛ lₜ). destruct (envs_app _ _ _) as [Δ' |] eqn:HΔ'; last done.
-    iApply Hsim.
-    iApply (envs_app_sound with "HΔ"); first done. simpl. auto with iFrame.
-  Qed.
-
-  Lemma tac_simv_constrₛ1 K constr e1 e2 e Φ Δ :
-    envs_entails Δ (SIM K @@ let: e1 in let: e2.[ren (+1)] in &&constr $1 $0 ≳ e [[ X ]] [[ Φ ]]) →
-    envs_entails Δ (SIM K @@ &constr e1 e2 ≳ e [[ X ]] [[ Φ ]]).
-  Proof.
-    rewrite definition.simv_unseal /definition.simv_def.
-    rewrite envs_entails_unseal sim_bind_invₛ sim_constrₛ1 sim_bindₛ //.
-  Qed.
-  Lemma tac_simv_constrₛ2 K constr e1 e2 e Φ Δ :
-    envs_entails Δ (SIM K @@ let: e2 in let: e1.[ren (+1)] in &&constr $0 $1 ≳ e [[ X ]] [[ Φ ]]) →
-    envs_entails Δ (SIM K @@ &constr e1 e2 ≳ e [[ X ]] [[ Φ ]]).
-  Proof.
-    rewrite definition.simv_unseal /definition.simv_def.
-    rewrite envs_entails_unseal sim_bind_invₛ sim_constrₛ2 sim_bindₛ //.
-  Qed.
-  Lemma tac_simv_constrₜ e K constr e1 e2 Φ Δ :
-    envs_entails Δ (SIM e ≳ K @@ let: e1 in let: e2.[ren (+1)] in &&constr $1 $0 [[ X ]] [[ Φ ]]) →
-    envs_entails Δ (SIM e ≳ K @@ let: e2 in let: e1.[ren (+1)] in &&constr $0 $1 [[ X ]] [[ Φ ]]) →
-    envs_entails Δ (SIM e ≳ K @@ &constr e1 e2 [[ X ]] [[ Φ ]]).
-  Proof.
-    rewrite definition.simv_unseal /definition.simv_def.
-    rewrite envs_entails_unseal => Hsim1 Hsim2.
-    rewrite -sim_bindₜ -sim_constrₜ -!sim_bind_invₜ.
-    apply bi.and_intro; done.
-  Qed.
-
-  Lemma tac_simv_loadₛ id p K l idx v e Φ Δ :
-    envs_lookup id Δ = Some (p, (l +ₗ idx) ↦ₛ v)%I →
-    envs_entails Δ (SIM K @@ #v ≳ e [[ X ]] [[ Φ ]]) →
-    envs_entails Δ (SIM K @@ ![idx] l ≳ e [[ X ]] [[ Φ ]]).
-  Proof.
-    rewrite definition.simv_unseal /definition.simv_def.
-    rewrite envs_entails_unseal => Hlookup Hsim.
-    rewrite envs_lookup_split // -sim_bindₛ Hsim.
-    destruct p; simpl;
-      [iIntros "(#Hl & Hsim)" | iIntros "(Hl & Hsim)"];
-      iApply (sim_loadₛ with "Hl"); iIntros;
-      iApply sim_bind_invₛ;
-      iApply ("Hsim" with "[$]").
-  Qed.
-  Lemma tac_simv_loadₜ id p e K l idx v Φ Δ :
-    envs_lookup id Δ = Some (p, (l +ₗ idx) ↦ₜ v)%I →
-    envs_entails Δ (SIM e ≳ K @@ #v [[ X ]] [[ Φ ]]) →
-    envs_entails Δ (SIM e ≳ K @@ ![idx] l [[ X ]] [[ Φ ]]).
-  Proof.
-    rewrite definition.simv_unseal /definition.simv_def.
-    rewrite envs_entails_unseal => Hlookup Hsim.
-    rewrite envs_lookup_split // -sim_bindₜ Hsim.
-    destruct p; simpl;
-      [iIntros "(#Hl & Hsim)" | iIntros "(Hl & Hsim)"];
-      iApply (sim_loadₜ with "Hl"); iIntros;
-      iApply sim_bind_invₜ;
-      iApply ("Hsim" with "[$]").
-  Qed.
-  Lemma tac_simv_load id Kₛ lₛ idxₛ Kₜ lₜ idxₜ Φ Δ :
-    envs_entails Δ (Loc lₛ ≈ Loc lₜ) →
-    envs_entails Δ (Index idxₛ ≈ Index idxₜ) →
-    ( ∀ vₛ vₜ,
-      match envs_app true (Esnoc Enil id (vₛ ≈ vₜ)) Δ with
+          envs_entails Δ' (SIM K @@ #() ≳ e [[ X ]] [[ Φ ]])
+      end →
+      envs_entails Δ (SIM K @@ #l <-[idx]- v ≳ e [[ X ]] [[ Φ ]]).
+    Proof.
+      rewrite definition.simv_unseal /definition.simv_def.
+      apply tac_sim_storeₛ.
+    Qed.
+    Lemma tac_simv_storeₜ id p e K l idx v w Φ Δ :
+      envs_lookup id Δ = Some (p, (l +ₗ idx) ↦ₜ w)%I →
+      match envs_replace id p false (Esnoc Enil id ((l +ₗ idx) ↦ₜ v)) Δ with
       | None =>
           False
       | Some Δ' =>
-          envs_entails Δ' (SIM Kₛ @@ #vₛ ≳ Kₜ @@ #vₜ [[ X ]] [[ Φ ]])
-      end
-    ) →
-    envs_entails Δ (SIM Kₛ @@ ![idxₛ] lₛ ≳ Kₜ @@ ![idxₜ] lₜ [[ X ]] [[ Φ ]]).
-  Proof.
-    rewrite definition.simv_unseal /definition.simv_def.
-    rewrite envs_entails_unseal => Hl Hidx Hsim.
-    iIntros "HΔ".
-    iDestruct (Hl with "HΔ") as "#Hl".
-    iDestruct (Hidx with "HΔ") as "#Hidx".
-    iApply sim_bind.
-    iApply (sim_load with "Hl Hidx"). iIntros "%vₛ %vₜ #Hv".
-    specialize (Hsim vₛ vₜ). destruct (envs_app _ _ _) as [Δ' |] eqn:HΔ'; last done.
-    iApply sim_bind_inv. iApply Hsim.
-    iApply (envs_app_singleton_sound with "[HΔ] [Hv]"); naive_solver.
-  Qed.
+          envs_entails Δ' (SIM e ≳ K @@ #() [[ X ]] [[ Φ ]])
+      end →
+      envs_entails Δ (SIM e ≳ K @@ #l <-[idx]- v [[ X ]] [[ Φ ]]).
+    Proof.
+      rewrite definition.simv_unseal /definition.simv_def.
+      apply tac_sim_storeₜ.
+    Qed.
+    Lemma tac_simv_store Kₛ vₛ1 vₛ2 vₛ3 Kₜ vₜ1 vₜ2 vₜ3 Φ Δ :
+      envs_entails Δ (vₛ1 ≈ vₜ1) →
+      envs_entails Δ (vₛ2 ≈ vₜ2) →
+      envs_entails Δ (vₛ3 ≈ vₜ3) →
+      envs_entails Δ (SIM Kₛ @@ #() ≳ Kₜ @@ #() [[ X ]] [[ Φ ]]) →
+      envs_entails Δ (SIM Kₛ @@ vₛ1 <-[vₛ2]- vₛ3 ≳ Kₜ @@ vₜ1 <-[vₜ2]- vₜ3 [[ X ]] [[ Φ ]]).
+    Proof.
+      rewrite definition.simv_unseal /definition.simv_def.
+      apply tac_sim_store.
+    Qed.
+  End simv.
+End sim_GS.
 
-  Lemma tac_simv_storeₛ id p K l idx v w e Φ Δ :
-    envs_lookup id Δ = Some (p, (l +ₗ idx) ↦ₛ w)%I →
-    match envs_replace id p false (Esnoc Enil id ((l +ₗ idx) ↦ₛ v)) Δ with
-    | None =>
-        False
-    | Some Δ' =>
-        envs_entails Δ' (SIM K @@ #() ≳ e [[ X ]] [[ Φ ]])
-    end →
-    envs_entails Δ (SIM K @@ #l <-[idx]- v ≳ e [[ X ]] [[ Φ ]]).
-  Proof.
-    rewrite definition.simv_unseal /definition.simv_def.
-    rewrite envs_entails_unseal => Hlookup Hsim.
-    destruct (envs_replace _ _ _ _) as [Δ' |] eqn:HΔ'; last done.
-    rewrite envs_replace_singleton_sound // Hsim.
-    rewrite bi.intuitionistically_if_elim /=.
-    rewrite sim_bind_invₛ -sim_bindₛ. apply bi.wand_elim_l', sim_storeₛ.
-  Qed.
-  Lemma tac_simv_storeₜ id p e K l idx v w Φ Δ :
-    envs_lookup id Δ = Some (p, (l +ₗ idx) ↦ₜ w)%I →
-    match envs_replace id p false (Esnoc Enil id ((l +ₗ idx) ↦ₜ v)) Δ with
-    | None =>
-        False
-    | Some Δ' =>
-        envs_entails Δ' (SIM e ≳ K @@ #() [[ X ]] [[ Φ ]])
-    end →
-    envs_entails Δ (SIM e ≳ K @@ #l <-[idx]- v [[ X ]] [[ Φ ]]).
-  Proof.
-    rewrite definition.simv_unseal /definition.simv_def.
-    rewrite envs_entails_unseal => Hlookup Hsim.
-    destruct (envs_replace _ _ _ _) as [Δ' |] eqn:HΔ'; last done.
-    rewrite envs_replace_singleton_sound // Hsim.
-    rewrite bi.intuitionistically_if_elim /=.
-    rewrite sim_bind_invₜ -sim_bindₜ. apply bi.wand_elim_l', sim_storeₜ.
-  Qed.
-  Lemma tac_simv_store Kₛ vₛ1 vₛ2 vₛ3 Kₜ vₜ1 vₜ2 vₜ3 Φ Δ :
-    envs_entails Δ (vₛ1 ≈ vₜ1) →
-    envs_entails Δ (vₛ2 ≈ vₜ2) →
-    envs_entails Δ (vₛ3 ≈ vₜ3) →
-    envs_entails Δ (SIM Kₛ @@ #() ≳ Kₜ @@ #() [[ X ]] [[ Φ ]]) →
-    envs_entails Δ (SIM Kₛ @@ vₛ1 <-[vₛ2]- vₛ3 ≳ Kₜ @@ vₜ1 <-[vₜ2]- vₜ3 [[ X ]] [[ Φ ]]).
-  Proof.
-    rewrite definition.simv_unseal /definition.simv_def.
-    rewrite envs_entails_unseal => Hv1 Hv2 Hv3 Hsim.
-    iIntros "HΔ".
-    iDestruct (Hv1 with "HΔ") as "#Hv1".
-    iDestruct (Hv2 with "HΔ") as "#Hv2".
-    iDestruct (Hv3 with "HΔ") as "#Hv3".
-    iApply sim_bind. iApply (sim_store with "Hv1 Hv2 Hv3"). iApply (Hsim with "HΔ").
-  Qed.
-End sim.
-
-(* #[local] *)
-Ltac expr_decompose e tac :=
+#[local] Ltac expr_decompose e tac :=
   let rec go K e :=
     let go k e := go (k :: K) e in
     match e with
@@ -283,27 +427,25 @@ Ltac expr_decompose e tac :=
     end
   in
   go (∅ : ectx) e.
-(* #[local] *)
-Tactic Notation "expr_decompose" "[" open_constr(eₛ) open_constr(eₜ) "]" tactic3(tac) :=
+#[local] Tactic Notation "expr_decompose" "[" open_constr(eₛ) open_constr(eₜ) "]" tactic3(tac) :=
   expr_decompose eₛ ltac:(fun Kₛ eₛ' =>
     expr_decompose eₜ ltac:(fun Kₜ eₜ' =>
       tac Kₛ eₛ' Kₜ eₜ'
     )
   ).
 
-Tactic Notation "simv_finish" :=
-  simv_finish with asimpl.
+Tactic Notation "sim_finish" :=
+  sim_finish with asimpl.
 
-Ltac simv_asimpl :=
-  simv_eval (asimpl; simpl).
-Ltac simv_asimplₛ :=
-  simv_evalₛ (asimpl; simpl).
-Ltac simv_asimplₜ :=
-  simv_evalₜ (asimpl; simpl).
+Ltac sim_asimpl :=
+  sim_eval (asimpl; simpl).
+Ltac sim_asimplₛ :=
+  sim_evalₛ (asimpl; simpl).
+Ltac sim_asimplₜ :=
+  sim_evalₜ (asimpl; simpl).
 
-(* #[local] *)
-Ltac simv_focalizeₛ e_foc tac_succ tac_fail :=
-  on_simv ltac:(fun _ _ _ e _ =>
+#[local] Ltac sim_focalizeₛ e_foc tac_succ tac_fail :=
+  on_sim_or_simv' ltac:(fun _ _ _ e _ =>
     tryif
       expr_decompose e ltac:(fun K e' =>
         unify e' e_foc;
@@ -313,9 +455,8 @@ Ltac simv_focalizeₛ e_foc tac_succ tac_fail :=
       tac_fail e
     )
   ).
-(* #[local] *)
-Ltac simv_focalizeₜ e_foc tac_succ tac_fail :=
-  on_simv ltac:(fun _ _ _ _ e =>
+#[local] Ltac sim_focalizeₜ e_foc tac_succ tac_fail :=
+  on_sim_or_simv' ltac:(fun _ _ _ _ e =>
     tryif
       expr_decompose e ltac:(fun K e' =>
         unify e' e_foc;
@@ -325,9 +466,8 @@ Ltac simv_focalizeₜ e_foc tac_succ tac_fail :=
       tac_fail e
     )
   ).
-(* #[local] *)
-Ltac simv_focalize e_focₛ e_focₜ tac_succ tac_fail :=
-  on_simv ltac:(fun _ _ _ eₛ eₜ =>
+#[local] Ltac sim_focalize e_focₛ e_focₜ tac_succ tac_fail :=
+  on_sim_or_simv' ltac:(fun _ _ _ eₛ eₜ =>
     tryif
       expr_decompose eₛ ltac:(fun Kₛ eₛ' =>
         unify eₛ' e_focₛ;
@@ -341,28 +481,20 @@ Ltac simv_focalize e_focₛ e_focₜ tac_succ tac_fail :=
     )
   ).
 
-Tactic Notation "simv_bindₛ" open_constr(e_foc) :=
-  simv_focalizeₛ e_foc
-    ltac:(fun K =>
-      simv_bind_coreₛ K
-    )
-    ltac:(fun e =>
-      fail "simv_bindₛ: cannot find" e_foc "in source" e
-    ).
-Tactic Notation "simv_bindₛ" :=
-  simv_bindₛ _.
-Tactic Notation "simv_bindₜ" open_constr(e_foc) :=
-  simv_focalizeₜ e_foc
-    ltac:(fun K =>
-      simv_bind_coreₜ K
-    )
-    ltac:(fun e =>
-      fail "simv_bindₜ: cannot find" e_foc "in target" e
-    ).
-Tactic Notation "simv_bindₜ" :=
-  simv_bindₜ _.
-Tactic Notation "simv_bind" open_constr(e_focₛ) open_constr(e_focₜ) :=
-  on_simv ltac:(fun _ _ _ eₛ eₜ =>
+Tactic Notation "sim_bindₛ" open_constr(e_foc) :=
+  sim_focalizeₛ e_foc
+    ltac:(fun K => sim_bind_coreₛ K)
+    ltac:(fun e => fail "sim_bindₛ: cannot find" e_foc "in source" e).
+Tactic Notation "sim_bindₛ" :=
+  sim_bindₛ _.
+Tactic Notation "sim_bindₜ" open_constr(e_foc) :=
+  sim_focalizeₜ e_foc
+    ltac:(fun K => sim_bind_coreₜ K)
+    ltac:(fun e => fail "sim_bindₜ: cannot find" e_foc "in target" e).
+Tactic Notation "sim_bindₜ" :=
+  sim_bindₜ _.
+Tactic Notation "sim_bind" open_constr(e_focₛ) open_constr(e_focₜ) :=
+  on_sim ltac:(fun _ _ _ eₛ eₜ =>
     let Kₛ := open_constr:(_) in
     expr_decompose eₛ ltac:(fun Kₛ' eₛ' =>
       unify eₛ' e_focₛ;
@@ -373,129 +505,127 @@ Tactic Notation "simv_bind" open_constr(e_focₛ) open_constr(e_focₜ) :=
       unify eₜ' e_focₜ;
       unify Kₜ' Kₜ
     );
-    simv_bind_core Kₛ Kₜ
+    sim_bind_core Kₛ Kₜ
   ).
-Tactic Notation "simv_bind" :=
-  simv_bind _ _.
+Tactic Notation "sim_bind" :=
+  sim_bind _ _.
 
-Tactic Notation "simv_pureₛ" open_constr(e_foc) :=
-  simv_focalizeₛ e_foc
-    ltac:(fun K =>
-      simv_pure_coreₛ K
-    )
-    ltac:(fun e =>
-      fail "simv_pureₛ: cannot find" e_foc "in source" e "or" e_foc "is not a redex"
-    ).
-Tactic Notation "simv_pureₛ" :=
-  simv_pureₛ _.
-Ltac simv_puresₛ :=
-  repeat (simv_pureₛ; []) || simv_finish.
-Tactic Notation "simv_pureₜ" open_constr(e_foc) :=
-  simv_focalizeₜ e_foc
-    ltac:(fun K =>
-      simv_pure_coreₜ K
-    )
-    ltac:(fun e =>
-      fail "simv_pureₜ: cannot find" e_foc "in target" e "or" e_foc "is not a redex"
-    ).
-Tactic Notation "simv_pureₜ" :=
-  simv_pureₜ _.
-Ltac simv_puresₜ :=
-  repeat (simv_pureₜ; []) || simv_finish.
-Ltac simv_pures :=
-  simv_puresₜ; simv_puresₛ.
+Tactic Notation "sim_pureₛ" open_constr(e_foc) :=
+  sim_focalizeₛ e_foc
+    ltac:(fun K => sim_pure_coreₛ K)
+    ltac:(fun e => fail "sim_pureₛ: cannot find" e_foc "in source" e "or" e_foc "is not a redex").
+Tactic Notation "sim_pureₛ" :=
+  sim_pureₛ _.
+Ltac sim_puresₛ :=
+  repeat (sim_pureₛ; []) || sim_finish.
+Tactic Notation "sim_pureₜ" open_constr(e_foc) :=
+  sim_focalizeₜ e_foc
+    ltac:(fun K => sim_pure_coreₜ K)
+    ltac:(fun e => fail "sim_pureₜ: cannot find" e_foc "in target" e "or" e_foc "is not a redex").
+Tactic Notation "sim_pureₜ" :=
+  sim_pureₜ _.
+Ltac sim_puresₜ :=
+  repeat (sim_pureₜ; []) || sim_finish.
+Ltac sim_pures :=
+  sim_puresₜ; sim_puresₛ.
 
-#[local] Ltac simv_heap_bij_insert_core Htie Hsimilar :=
+#[local] Ltac sim_heap_bij_insert_core Htie Hsimilar :=
   iStartProof;
-  eapply (tac_simv_heap_bij_insert Htie _ Hsimilar);
+  eapply (tac_sim_heap_bij_insert Htie _ Hsimilar);
   [ iSolveTC
   | iAssumptionCore ||
     tryif is_evar Htie then (
-      fail "simv_heap_bij_insert: cannot find ? ⋈ ?"
+      fail "sim_heap_bij_insert: cannot find ? ⋈ ?"
     ) else (
-      fail "simv_heap_bij_insert: cannot find" Htie ": ? ⋈ ?"
+      fail "sim_heap_bij_insert: cannot find" Htie ": ? ⋈ ?"
     )
   | pm_reduce;
     tryif goal_is_false then (
-      fail "simv_heap_bij_insert:" Hsimilar "not fresh"
+      fail "sim_heap_bij_insert:" Hsimilar "not fresh"
     ) else (
-      try simv_finish
+      try sim_finish
     )
   ].
-Tactic Notation "simv_heap_bij_insert" open_constr(Htie) "as" constr(Hsimilar) :=
-  simv_heap_bij_insert_core Htie Hsimilar.
-Tactic Notation "simv_heap_bij_insert" open_constr(Htie) :=
-  simv_heap_bij_insert Htie as Htie.
-Tactic Notation "simv_heap_bij_insert" "as" constr(Hsimilar) :=
-  simv_heap_bij_insert _ as Hsimilar.
-Tactic Notation "simv_heap_bij_insert" :=
+Tactic Notation "sim_heap_bij_insert" open_constr(Htie) "as" constr(Hsimilar) :=
+  sim_heap_bij_insert_core Htie Hsimilar.
+Tactic Notation "sim_heap_bij_insert" open_constr(Htie) :=
+  sim_heap_bij_insert Htie as Htie.
+Tactic Notation "sim_heap_bij_insert" "as" constr(Hsimilar) :=
+  sim_heap_bij_insert _ as Hsimilar.
+Tactic Notation "sim_heap_bij_insert" :=
   let Htie := open_constr:(_) in
-  simv_heap_bij_insert_core Htie Htie.
+  sim_heap_bij_insert_core Htie Htie.
 
-Tactic Notation "simv_constr_detₛ" "as" simple_intropattern(l) constr(Hl0) constr(Hl1) constr(Hl2) :=
-  simv_pures;
+Tactic Notation "sim_constr_detₛ" "as" simple_intropattern(l) constr(Hl0) constr(Hl1) constr(Hl2) :=
+  sim_pures;
   let e_foc := open_constr:(ConstrDet _ (Val _) (Val _)) in
-  simv_focalizeₛ e_foc
+  sim_focalizeₛ e_foc
     ltac:(fun K =>
-      eapply (tac_simv_constr_detₛ _ Hl0 Hl1 Hl2 K)
+      on_sim_or_simv
+        ltac:(fun _ _ _ _ _ => eapply (tac_sim_constr_detₛ _ Hl0 Hl1 Hl2 K))
+        ltac:(fun _ _ _ _ _ => eapply (tac_simv_constr_detₛ _ Hl0 Hl1 Hl2 K))
     )
     ltac:(fun e =>
-      fail "simv_constr_detₛ: cannot find" e_foc "in source" e
+      fail "sim_constr_detₛ: cannot find" e_foc "in source" e
     );
   tryif intros l then idtac else (
-    fail "simv_constr_detₛ:" l "not fresh"
+    fail "sim_constr_detₛ:" l "not fresh"
   );
   pm_reduce;
   tryif goal_is_false then (
-    fail "simv_constr_detₛ:" Hl0 "or" Hl1 "or" Hl2 "not fresh"
+    fail "sim_constr_detₛ:" Hl0 "or" Hl1 "or" Hl2 "not fresh"
   ) else (
-    simv_finish
+    sim_finish
   ).
-Tactic Notation "simv_constr_detₛ" "as" simple_intropattern(l) :=
+Tactic Notation "sim_constr_detₛ" "as" simple_intropattern(l) :=
   let Hl0 := iFresh in
   let Hl1 := iFresh in
   let Hl2 := iFresh in
-  simv_constr_detₛ as l Hl0 Hl1 Hl2.
-Tactic Notation "simv_constr_detₛ" :=
+  sim_constr_detₛ as l Hl0 Hl1 Hl2.
+Tactic Notation "sim_constr_detₛ" :=
   let l := fresh "lₛ" in
-  simv_constr_detₛ as l.
-Tactic Notation "simv_constr_detₜ" "as" simple_intropattern(l) constr(Hl0) constr(Hl1) constr(Hl2) :=
-  simv_pures;
+  sim_constr_detₛ as l.
+Tactic Notation "sim_constr_detₜ" "as" simple_intropattern(l) constr(Hl0) constr(Hl1) constr(Hl2) :=
+  sim_pures;
   let e_foc := open_constr:(ConstrDet _ (Val _) (Val _)) in
-  simv_focalizeₜ e_foc
+  sim_focalizeₜ e_foc
     ltac:(fun K =>
-      eapply (tac_simv_constr_detₜ _ Hl0 Hl1 Hl2 _ K)
+      on_sim_or_simv
+        ltac:(fun _ _ _ _ _ => eapply (tac_sim_constr_detₜ _ Hl0 Hl1 Hl2 _ K))
+        ltac:(fun _ _ _ _ _ => eapply (tac_simv_constr_detₜ _ Hl0 Hl1 Hl2 _ K))
     )
     ltac:(fun e =>
-      fail "simv_constr_detₜ: cannot find" e_foc "in target" e
+      fail "sim_constr_detₜ: cannot find" e_foc "in target" e
     );
   tryif intros l then idtac else (
-    fail "simv_constr_detₜ:" l "not fresh"
+    fail "sim_constr_detₜ:" l "not fresh"
   );
   pm_reduce;
   tryif goal_is_false then (
-    fail "simv_constr_detₜ:" Hl0 "or" Hl1 "or" Hl2 "not fresh"
+    fail "sim_constr_detₜ:" Hl0 "or" Hl1 "or" Hl2 "not fresh"
   ) else (
-    simv_finish
+    sim_finish
   ).
-Tactic Notation "simv_constr_detₜ" "as" simple_intropattern(l) :=
+Tactic Notation "sim_constr_detₜ" "as" simple_intropattern(l) :=
   let Hl0 := iFresh in
   let Hl1 := iFresh in
   let Hl2 := iFresh in
-  simv_constr_detₜ as l Hl0 Hl1 Hl2.
-Tactic Notation "simv_constr_detₜ" :=
+  sim_constr_detₜ as l Hl0 Hl1 Hl2.
+Tactic Notation "sim_constr_detₜ" :=
   let l := fresh "lₜ" in
-  simv_constr_detₜ as l.
-Tactic Notation "simv_constr_det" "as" simple_intropattern(lₛ) simple_intropattern(lₜ) constr(Hl) :=
-  simv_pures;
+  sim_constr_detₜ as l.
+Tactic Notation "sim_constr_det" "as" simple_intropattern(lₛ) simple_intropattern(lₜ) constr(Hl) :=
+  sim_pures;
   let e_focₛ := open_constr:(ConstrDet _ (Val _) (Val _)) in
   let e_focₜ := open_constr:(ConstrDet _ (Val _) (Val _)) in
-  simv_focalize e_focₛ e_focₜ
+  sim_focalize e_focₛ e_focₜ
     ltac:(fun Kₛ Kₜ =>
-      eapply (tac_simv_constr_det _ Hl _ Kₛ _ _ Kₜ)
+      on_sim_or_simv
+        ltac:(fun _ _ _ _ _ => eapply (tac_sim_constr_det _ Hl _ Kₛ _ _ Kₜ))
+        ltac:(fun _ _ _ _ _ => eapply (tac_simv_constr_det _ Hl _ Kₛ _ _ Kₜ))
     )
     ltac:(fun eₛ eₜ =>
-      fail "simv_constr_det: cannot find" e_focₛ "in source" eₛ "or" e_focₜ "in target" eₜ
+      fail "sim_constr_det: cannot find" e_focₛ "in source" eₛ "or" e_focₜ "in target" eₜ
     );
   [ try done
   | try done
@@ -503,97 +633,109 @@ Tactic Notation "simv_constr_det" "as" simple_intropattern(lₛ) simple_intropat
       tryif intros lₜ then (
         pm_reduce;
         tryif goal_is_false then (
-          fail "simv_constr_det:" Hl "not fresh"
+          fail "sim_constr_det:" Hl "not fresh"
         ) else (
-          simv_finish
+          sim_finish
         )
       ) else (
-        fail "simv_constr_det:" lₜ "not fresh"
+        fail "sim_constr_det:" lₜ "not fresh"
       )
     ) else (
-      fail "simv_constr_det:" lₛ "not fresh"
+      fail "sim_constr_det:" lₛ "not fresh"
     )
   ].
-Tactic Notation "simv_constr_det" "as" simple_intropattern(lₛ) simple_intropattern(lₜ) :=
+Tactic Notation "sim_constr_det" "as" simple_intropattern(lₛ) simple_intropattern(lₜ) :=
   let Hl := iFresh in
-  simv_constr_det as lₜ lₛ Hl.
-Tactic Notation "simv_constr_det" :=
-  simv_constr_det as ? ?.
+  sim_constr_det as lₜ lₛ Hl.
+Tactic Notation "sim_constr_det" :=
+  sim_constr_det as ? ?.
 
-Ltac simv_constrₛ1 :=
-  simv_pures;
+Ltac sim_constrₛ1 :=
+  sim_pures;
   let e_foc := open_constr:(Constr _ _ _) in
-  simv_focalizeₛ e_foc
+  sim_focalizeₛ e_foc
     ltac:(fun K =>
-      eapply (tac_simv_constrₛ1 _ K)
+      on_sim_or_simv
+        ltac:(fun _ _ _ _ _ => eapply (tac_sim_constrₛ1 _ K))
+        ltac:(fun _ _ _ _ _ => eapply (tac_simv_constrₛ1 _ K))
     )
     ltac:(fun e =>
-      fail "simv_constrₛ1: cannot find" e_foc "in source" e
+      fail "sim_constrₛ1: cannot find" e_foc "in source" e
     );
-  simv_finish.
-Ltac simv_constrₛ2 :=
-  simv_pures;
+  sim_finish.
+Ltac sim_constrₛ2 :=
+  sim_pures;
   let e_foc := open_constr:(Constr _ _ _) in
-  simv_focalizeₛ e_foc
+  sim_focalizeₛ e_foc
     ltac:(fun K =>
-      eapply (tac_simv_constrₛ2 _ K)
+      on_sim_or_simv
+        ltac:(fun _ _ _ _ _ => eapply (tac_sim_constrₛ2 _ K))
+        ltac:(fun _ _ _ _ _ => eapply (tac_simv_constrₛ2 _ K))
     )
     ltac:(fun e =>
-      fail "simv_constrₛ2: cannot find" e_foc "in source" e
+      fail "sim_constrₛ2: cannot find" e_foc "in source" e
     );
-  simv_finish.
-Ltac simv_constrₜ :=
-  simv_pures;
+  sim_finish.
+Ltac sim_constrₜ :=
+  sim_pures;
   let e_foc := open_constr:(Constr _ _ _) in
-  simv_focalizeₜ e_foc
+  sim_focalizeₜ e_foc
     ltac:(fun K =>
-      eapply (tac_simv_constrₜ _ _ K)
+      on_sim_or_simv
+        ltac:(fun _ _ _ _ _ => eapply (tac_sim_constrₜ _ _ K))
+        ltac:(fun _ _ _ _ _ => eapply (tac_simv_constrₜ _ _ K))
     )
     ltac:(fun e =>
-      fail "simv_constrₜ: cannot find" e_foc "in target" e
+      fail "sim_constrₜ: cannot find" e_foc "in target" e
     );
-  simv_finish.
+  sim_finish.
 
-Tactic Notation "simv_loadₛ" :=
-  simv_pures;
+Tactic Notation "sim_loadₛ" :=
+  sim_pures;
   let e_foc := open_constr:(Load (Val (Loc _)) (Val (Index _))) in
-  simv_focalizeₛ e_foc
+  sim_focalizeₛ e_foc
     ltac:(fun K =>
-      eapply (tac_simv_loadₛ _ _ _ K)
+      on_sim_or_simv
+        ltac:(fun _ _ _ _ _ => eapply (tac_sim_loadₛ _ _ _ K))
+        ltac:(fun _ _ _ _ _ => eapply (tac_simv_loadₛ _ _ _ K))
     )
     ltac:(fun e =>
-      fail "simv_loadₛ: cannot find" e_foc "in source" e
+      fail "sim_loadₛ: cannot find" e_foc "in source" e
     );
   [ iAssumptionCore ||
     let l := match goal with |- _ = Some (_, mapstoₛ ?l _ _) => l end in
-    fail "simv_loadₛ: cannot find" l "↦ₛ ?"
-  | simv_finish
+    fail "sim_loadₛ: cannot find" l "↦ₛ ?"
+  | sim_finish
   ].
-Tactic Notation "simv_loadₜ" :=
-  simv_pures;
+Tactic Notation "sim_loadₜ" :=
+  sim_pures;
   let e_foc := open_constr:(Load (Val (Loc _)) (Val (Index _))) in
-  simv_focalizeₜ e_foc
+  sim_focalizeₜ e_foc
     ltac:(fun K =>
-      eapply (tac_simv_loadₜ _ _ _ _ K)
+    on_sim_or_simv
+      ltac:(fun _ _ _ _ _ => eapply (tac_sim_loadₜ _ _ _ _ K))
+      ltac:(fun _ _ _ _ _ => eapply (tac_simv_loadₜ _ _ _ _ K))
     )
     ltac:(fun e =>
-      fail "simv_loadₜ: cannot find" e_foc "in target" e
+      fail "sim_loadₜ: cannot find" e_foc "in target" e
     );
   [ iAssumptionCore ||
     let l := match goal with |- _ = Some (_, mapstoₜ ?l _ _) => l end in
-    fail "simv_loadₜ: cannot find" l "↦ₜ ?"
-  | simv_finish
+    fail "sim_loadₜ: cannot find" l "↦ₜ ?"
+  | sim_finish
   ].
-Tactic Notation "simv_load" "as" simple_intropattern(vₛ) simple_intropattern(vₜ) constr(Hv) :=
-  simv_pures;
+Tactic Notation "sim_load" "as" simple_intropattern(vₛ) simple_intropattern(vₜ) constr(Hv) :=
+  sim_pures;
   let e_focₛ := open_constr:(Load (Val (Loc _)) (Val (Index _))) in
   let e_focₜ := open_constr:(Load (Val (Loc _)) (Val (Index _))) in
-  simv_focalize e_focₛ e_focₜ
+  sim_focalize e_focₛ e_focₜ
     ltac:(fun Kₛ Kₜ =>
-      eapply (tac_simv_load _ Hv Kₛ _ _ Kₜ)
+      on_sim_or_simv
+        ltac:(fun _ _ _ _ _ => eapply (tac_sim_load _ Hv Kₛ _ _ Kₜ))
+        ltac:(fun _ _ _ _ _ => eapply (tac_simv_load _ Hv Kₛ _ _ Kₜ))
     )
     ltac:(fun eₛ eₜ =>
-      fail "simv_load: cannot find" e_focₛ "in source" eₛ "or" e_focₜ "in target" eₜ
+      fail "sim_load: cannot find" e_focₛ "in source" eₛ "or" e_focₜ "in target" eₜ
     );
   [ try done
   | try done
@@ -601,95 +743,101 @@ Tactic Notation "simv_load" "as" simple_intropattern(vₛ) simple_intropattern(v
       tryif intros vₜ then (
         pm_reduce;
         tryif goal_is_false then (
-          fail "simv_load:" Hv "not fresh"
+          fail "sim_load:" Hv "not fresh"
         ) else (
-          simv_finish
+          sim_finish
         )
       ) else (
-        fail "simv_load:" vₜ "not fresh"
+        fail "sim_load:" vₜ "not fresh"
       )
     ) else (
-      fail "simv_load:" vₛ "not fresh"
+      fail "sim_load:" vₛ "not fresh"
     )
   ].
-Tactic Notation "simv_load" "as" simple_intropattern(vₛ) simple_intropattern(vₜ) :=
+Tactic Notation "sim_load" "as" simple_intropattern(vₛ) simple_intropattern(vₜ) :=
   let Hv := iFresh in
-  simv_load as vₛ vₜ Hv.
-Tactic Notation "simv_load" :=
-  simv_load as ? ?.
+  sim_load as vₛ vₜ Hv.
+Tactic Notation "sim_load" :=
+  sim_load as ? ?.
 
-Ltac simv_storeₛ :=
-  simv_pures;
+Ltac sim_storeₛ :=
+  sim_pures;
   let e_foc := open_constr:(Store (Val (Loc _)) (Val (Index _)) (Val _)) in
-  simv_focalizeₛ e_foc
+  sim_focalizeₛ e_foc
     ltac:(fun K =>
-      eapply (tac_simv_storeₛ _ _ _ K)
+      on_sim_or_simv
+        ltac:(fun _ _ _ _ _ => eapply (tac_sim_storeₛ _ _ _ K))
+        ltac:(fun _ _ _ _ _ => eapply (tac_simv_storeₛ _ _ _ K))
     )
     ltac:(fun e =>
-      fail "simv_storeₛ: cannot find" e_foc "in source" e
+      fail "sim_storeₛ: cannot find" e_foc "in source" e
     );
   [ iAssumptionCore ||
     let l := match goal with |- _ = Some (_, mapstoₛ ?l _ _) => l end in
-    fail "simv_storeₛ: cannot find" l "↦ₛ ?"
-  | pm_reduce; simv_finish
+    fail "sim_storeₛ: cannot find" l "↦ₛ ?"
+  | pm_reduce; sim_finish
   ].
-Ltac simv_storeₜ :=
-  simv_pures;
+Ltac sim_storeₜ :=
+  sim_pures;
   let e_foc := open_constr:(Store (Val (Loc _)) (Val (Index _)) (Val _)) in
-  simv_focalizeₜ e_foc
+  sim_focalizeₜ e_foc
     ltac:(fun K =>
-      eapply (tac_simv_storeₜ _ _ _ _ K)
+      on_sim_or_simv
+        ltac:(fun _ _ _ _ _ => eapply (tac_sim_storeₜ _ _ _ _ K))
+        ltac:(fun _ _ _ _ _ => eapply (tac_simv_storeₜ _ _ _ _ K))
     )
     ltac:(fun e =>
-      fail "simv_storeₜ: cannot find" e_foc "in source" e
+      fail "sim_storeₜ: cannot find" e_foc "in source" e
     );
   [ iAssumptionCore ||
     let l := match goal with |- _ = Some (_, mapstoₜ ?l _ _) => l end in
-    fail "simv_storeₜ: cannot find" l "↦ₜ ?"
-  | pm_reduce; simv_finish
+    fail "sim_storeₜ: cannot find" l "↦ₜ ?"
+  | pm_reduce; sim_finish
   ].
-Ltac simv_store :=
-  simv_pures;
+Ltac sim_store :=
+  sim_pures;
   let e_focₜ := open_constr:(Store (Val (Loc _)) (Val (Index _)) (Val _)) in
   let e_focₛ := open_constr:(Store (Val (Loc _)) (Val (Index _)) (Val _)) in
-  simv_focalize e_focₜ e_focₛ
+  sim_focalize e_focₜ e_focₛ
     ltac:(fun Kₛ Kₜ =>
-      eapply (tac_simv_store _ Kₛ _ _ _ Kₜ)
+      on_sim_or_simv
+        ltac:(fun _ _ _ _ _ => eapply (tac_sim_store _ Kₛ _ _ _ Kₜ))
+        ltac:(fun _ _ _ _ _ => eapply (tac_simv_store _ Kₛ _ _ _ Kₜ))
     )
     ltac:(fun eₛ eₜ =>
-      fail "simv_store: cannot find" e_focₛ "in source" eₛ "or" e_focₜ "in target" eₜ
+      fail "sim_store: cannot find" e_focₛ "in source" eₛ "or" e_focₜ "in target" eₜ
     );
   [ try done
   | try done
   | try done
-  | simv_finish
+  | sim_finish
   ].
 
-Tactic Notation "simv_apply" open_constr(H) :=
-  on_simv ltac:(fun _ _ _ eₛ eₜ =>
+Tactic Notation "sim_apply" open_constr(H) :=
+  on_sim_or_simv' ltac:(fun _ _ _ eₛ eₜ =>
     tryif
       iPoseProofCore H as false ltac:(fun H =>
         expr_decompose [eₛ eₜ] ltac:(fun Kₛ _ Kₜ _ =>
-          simv_bind_core Kₛ Kₜ;
+          sim_bind_core Kₛ Kₜ;
           iApplyHyp H;
           try done
         )
       )
     then idtac else (
       let P := type of H in
-      fail "simv_apply: cannot apply" H ":" P
+      fail "sim_apply: cannot apply" H ":" P
     )
   ).
-Tactic Notation "simv_smart_apply" open_constr(H) :=
-  simv_pures;
-  simv_apply H.
+Tactic Notation "sim_smart_apply" open_constr(H) :=
+  sim_pures;
+  sim_apply H.
 
-Tactic Notation "simv_mono" open_constr(H) :=
-  on_simv ltac:(fun _ _ _ eₛ eₜ =>
+Tactic Notation "sim_mono" open_constr(H) :=
+  on_sim_or_simv' ltac:(fun _ _ _ eₛ eₜ =>
     tryif
       iPoseProofCore H as false ltac:(fun H =>
         expr_decompose [eₛ eₜ] ltac:(fun Kₛ _ Kₜ _ =>
-          simv_bind_core Kₛ Kₜ;
+          sim_bind_core Kₛ Kₜ;
           let H_sel :=
             open_constr:(
               spec_patterns.SGoal (
@@ -698,7 +846,9 @@ Tactic Notation "simv_mono" open_constr(H) :=
               )
             )
           in
-          iApply (simv_mono' with H_sel);
+          on_sim_or_simv
+            ltac:(fun _ _ _ _ _ => iApply (sim_mono' with H_sel))
+            ltac:(fun _ _ _ _ _ => iApply (simv_mono' with H_sel));
           [ iApplyHyp H; try done
           | try solve [done | iIntros "% % ? //"]
           ]
@@ -706,9 +856,9 @@ Tactic Notation "simv_mono" open_constr(H) :=
       )
     then idtac else (
       let P := type of H in
-      fail "simv_mono: cannot apply" H ":" P
+      fail "sim_mono: cannot apply" H ":" P
     )
   ).
-Tactic Notation "simv_smart_mono" open_constr(H) :=
-  simv_pures;
-  simv_mono H.
+Tactic Notation "sim_smart_mono" open_constr(H) :=
+  sim_pures;
+  sim_mono H.
